src/HOL/Nominal/Examples/Crary.thy
@@ -8,15 +8,60 @@
 (* The formalisation was done by Julien Narboux and   *)
 (* Christian Urban                                    *)
 
+(*<*)
 theory Crary
-  imports "Nominal"
+  imports "../Nominal"
 begin
 
+(* We put this def here because of some incompatibility of LatexSugar and Nominal *)
+
+syntax (Rule output)
+  "==>" :: "prop \<Rightarrow> prop \<Rightarrow> prop"
+  ("\<^raw:\mbox{}\inferrule{\mbox{>_\<^raw:}}>\<^raw:{\mbox{>_\<^raw:}}>")
+
+  "_bigimpl" :: "asms \<Rightarrow> prop \<Rightarrow> prop"
+  ("\<^raw:\mbox{}\inferrule{>_\<^raw:}>\<^raw:{\mbox{>_\<^raw:}}>")
+
+  "_asms" :: "prop \<Rightarrow> asms \<Rightarrow> asms" 
+  ("\<^raw:\mbox{>_\<^raw:}\\>/ _")
+
+  "_asm" :: "prop \<Rightarrow> asms" ("\<^raw:\mbox{>_\<^raw:}>")
+
+syntax (IfThen output)
+  "==>" :: "prop \<Rightarrow> prop \<Rightarrow> prop"
+  ("\<^raw:{\rmfamily\upshape\normalsize{}>If\<^raw:\,}> _/ \<^raw:{\rmfamily\upshape\normalsize \,>then\<^raw:\,}>/ _.")
+  "_bigimpl" :: "asms \<Rightarrow> prop \<Rightarrow> prop"
+  ("\<^raw:{\rmfamily\upshape\normalsize{}>If\<^raw:\,}> _ /\<^raw:{\rmfamily\upshapce\normalsize \,>then\<^raw:\,}>/ _.")
+  "_asms" :: "prop \<Rightarrow> asms \<Rightarrow> asms" ("\<^raw:\mbox{>_\<^raw:}> /\<^raw:{\rmfamily\upshape\normalsize \,>and\<^raw:\,}>/ _")
+  "_asm" :: "prop \<Rightarrow> asms" ("\<^raw:\mbox{>_\<^raw:}>")
+
+syntax (IfThenNoBox output)
+  "==>" :: "prop \<Rightarrow> prop \<Rightarrow> prop"
+  ("\<^raw:{\rmfamily\upshape\normalsize{}>If\<^raw:\,}> _/ \<^raw:{\rmfamily\upshape\normalsize \,>then\<^raw:\,}>/ _.")
+  "_bigimpl" :: "asms \<Rightarrow> prop \<Rightarrow> prop"
+  ("\<^raw:{\rmfamily\upshape\normalsize{}>If\<^raw:\,}> _ /\<^raw:{\rmfamily\upshape\normalsize \,>then\<^raw:\,}>/ _.")
+  "_asms" :: "prop \<Rightarrow> asms \<Rightarrow> asms" ("_ /\<^raw:{\rmfamily\upshape\normalsize \,>and\<^raw:\,}>/ _")
+  "_asm" :: "prop \<Rightarrow> asms" ("_")
+
+
+(*>*)
+
+text {* 
+\section{Definition of the language} 
+\subsection{Definition of the terms and types} 
+
+First we define the type of atom names which will be used for binders.
+Each atom type is infinitely many atoms and equality is decidable. *}
+
 atom_decl name 
+
+text {* We define the datatype representing types. Although, It does not contain any binder we still use the \texttt{nominal\_datatype} command because the Nominal datatype package will prodive permutation functions and useful lemmas. *}
 
 nominal_datatype ty = TBase 
                     | TUnit 
                     | Arrow "ty" "ty" ("_\<rightarrow>_" [100,100] 100)
+
+text {* The datatype of terms contains a binder. The notation @{text "\<guillemotleft>name\<guillemotright> trm"} means that the name is bound inside trm. *}
 
 nominal_datatype trm = Unit
                      | Var "name"
@@ -24,27 +69,7 @@ nominal_datatype trm = Unit
                      | App "trm" "trm"
                      | Const "nat"
 
-(* The next 3 lemmas should be in the nominal library *)
-lemma eq_eqvt:
-  fixes pi::"name prm"
-  and   x::"'a::pt_name"
-  shows "pi\<bullet>(x=y) = (pi\<bullet>x=pi\<bullet>y)"
-  apply(simp add: perm_bool perm_bij)
-  done
-
-lemma in_eqvt:
-  fixes pi::"name prm"
-  and   x::"'a::pt_name"
-  assumes "x\<in>X"
-  shows "pi\<bullet>x \<in> pi\<bullet>X"
-  using assms by (perm_simp add: pt_set_bij1a[OF pt_name_inst, OF at_name_inst])
-
-lemma set_eqvt:
-  fixes pi::"name prm"
-  and   xs::"('a::pt_name) list"
-  shows "pi\<bullet>(set xs) = set (pi\<bullet>xs)"
-  by (perm_simp add: pt_list_set_pi[OF pt_name_inst])
-(* end of library *)
+text {* As the datatype of types does not contain any binder, the application of a permutation is the identity function. In the future, this will be automatically derived by the package. *}
 
 lemma perm_ty[simp]: 
   fixes T::"ty"
@@ -60,17 +85,23 @@ lemma fresh_ty[simp]:
 
 lemma ty_cases:
   fixes T::ty
-  shows "(\<exists> T1 T2. T=T1\<rightarrow>T2) \<or> T=TUnit \<or> T=TBase"
+  shows "(\<exists> T\<^isub>1 T\<^isub>2. T=T\<^isub>1\<rightarrow>T\<^isub>2) \<or> T=TUnit \<or> T=TBase"
 by (induct T rule:ty.induct_weak) (auto)
 
-text {* Size Functions *} 
+text {* 
+\subsection{Size functions}
+
+We define size functions for types and terms. As Isabelle allows overloading we can use the same notation for both functions.
+
+These function are automatically generated for non nominal datatypes. In the future, we need to extend the package to generate size function for nominal datatypes as well.
+ *} 
 
 instance ty :: size ..
 
 nominal_primrec
   "size (TBase) = 1"
   "size (TUnit) = 1"
-  "size (T1\<rightarrow>T2) = size T1 + size T2"
+  "size (T\<^isub>1\<rightarrow>T\<^isub>2) = size T\<^isub>1 + size T\<^isub>2"
 by (rule TrueI)+
 
 instance trm :: size ..
@@ -81,12 +112,10 @@ nominal_primrec
   "size (Lam [x].t) = size t + 1"
   "size (App t1 t2) = size t1 + size t2"
   "size (Const n) = 1"
-apply(finite_guess add: fs_name1 perm_nat_def)+
-apply(perm_full_simp add: perm_nat_def)
-apply(simp add: fs_name1)
+apply(finite_guess)+
 apply(rule TrueI)+
 apply(simp add: fresh_nat)+
-apply(fresh_guess add: fs_name1 perm_nat_def)+
+apply(fresh_guess)+
 done
 
 lemma ty_size_greater_zero[simp]:
@@ -94,56 +123,136 @@ lemma ty_size_greater_zero[simp]:
   shows "size T > 0"
 by (nominal_induct rule:ty.induct) (simp_all)
 
-text {* valid contexts *}
+text {* 
+\subsection{Typing}
 
+\subsubsection{Typing contexts}
+
+This section contains the definition and some properties of a typing context. As the concept of context often appears in the litterature and is general, we should in the future provide these lemmas in a library.
+
+\paragraph{Definition of the Validity of contexts}\strut\\
+
+First we define what valid contexts are. Informally a context is valid is it does not contains twice the same variable.
+
+We use the following two inference rules: *}
+
+(*<*)
 inductive2
   valid :: "(name \<times> 'a::pt_name) list \<Rightarrow> bool"
 where
     v_nil[intro]:  "valid []"
   | v_cons[intro]: "\<lbrakk>valid \<Gamma>;a\<sharp>\<Gamma>\<rbrakk> \<Longrightarrow> valid ((a,\<sigma>)#\<Gamma>)"
+(*>*)
 
-lemma valid_eqvt[eqvt]:
-  fixes   pi:: "name prm"
-  assumes a: "valid \<Gamma>"
-  shows "valid (pi\<bullet>\<Gamma>)"
-  using a
-  by (induct) (auto simp add: fresh_bij)
+text {*
+\begin{center}
+\isastyle
+@{thm[mode=Rule] v_nil[no_vars]}{\sc{v\_nil}}
+\qquad
+@{thm[mode=Rule] v_cons[no_vars]}{\sc{v\_cons}}
+\end{center}
+*} 
+
+text{* We generate the equivariance lemma for the relation \texttt{valid}. *}
+
+nominal_inductive valid
+
+text{* We obtain a lemma called \texttt{valid\_eqvt}:
+\begin{center} 
+@{thm[mode=IfThen] valid_eqvt}
+\end{center}
+*}
+
+
+text{* We generate the inversion lemma for non empty lists. We add the \texttt{elim} attribute to tell the automated tactics to use it.
+ *}
 
 inductive_cases2  
   valid_cons_elim_auto[elim]:"valid ((x,T)#\<Gamma>)"
 
-text {* typing judgements for terms *}
+text{*
+The generated theorem is the following:
+\begin{center}
+@{thm "valid_cons_elim_auto"[no_vars] }
+\end{center}
+*}
+
+text{* \paragraph{Lemmas about valid contexts} 
+ Now, we can prove two useful lemmas about valid contexts. 
+*}
+
+lemma fresh_context: 
+  fixes  \<Gamma> :: "(name\<times>ty) list"
+  and    a :: "name"
+  assumes "a\<sharp>\<Gamma>"
+  shows "\<not>(\<exists>\<tau>::ty. (a,\<tau>)\<in>set \<Gamma>)"
+using assms by (induct \<Gamma>, auto simp add: fresh_prod fresh_list_cons fresh_atm)
+
+lemma type_unicity_in_context:
+  fixes  \<Gamma> :: "(name\<times>ty)list"
+  and    pi:: "name prm"
+  and    a :: "name"
+  and    \<tau> :: "ty"
+  assumes "valid \<Gamma>" and "(x,T\<^isub>1) \<in> set \<Gamma>" and "(x,T\<^isub>2) \<in> set \<Gamma>"
+  shows "T\<^isub>1=T\<^isub>2"
+using assms by (induct \<Gamma>, auto dest!: fresh_context)
+
+text {* \paragraph{Definition of sub-contexts}
+
+The definition of sub context is standard. We do not use the subset definition to prevent the need for unfolding the definition. We include validity in the definition to shorten the statements.
+ *}
+
+
+abbreviation
+  "sub" :: "(name\<times>ty) list \<Rightarrow> (name\<times>ty) list \<Rightarrow> bool" (" _ \<lless> _ " [55,55] 55)
+where
+  "\<Gamma>\<^isub>1 \<lless> \<Gamma>\<^isub>2 \<equiv> (\<forall>a \<sigma>. (a,\<sigma>)\<in>set \<Gamma>\<^isub>1 \<longrightarrow> (a,\<sigma>)\<in>set \<Gamma>\<^isub>2) \<and> valid \<Gamma>\<^isub>2"
+
+text {* 
+\subsubsection{Definition of the typing relation}
+
+Now, we can define the typing judgements for terms. The rules are given in figure~\ref{typing}. *}
+
+(*<*)
 
 inductive2
   typing :: "(name\<times>ty) list\<Rightarrow>trm\<Rightarrow>ty\<Rightarrow>bool" (" _ \<turnstile> _ : _ " [60,60,60] 60) 
 where
   t_Var[intro]:   "\<lbrakk>valid \<Gamma>; (x,T)\<in>set \<Gamma>\<rbrakk>\<Longrightarrow> \<Gamma> \<turnstile> Var x : T"
-| t_App[intro]:   "\<lbrakk>\<Gamma> \<turnstile> e1 : T1\<rightarrow>T2; \<Gamma> \<turnstile> e2 : T1\<rbrakk>\<Longrightarrow> \<Gamma> \<turnstile> App e1 e2 : T2"
-| t_Lam[intro]:   "\<lbrakk>x\<sharp>\<Gamma>; (x,T1)#\<Gamma> \<turnstile> t : T2\<rbrakk> \<Longrightarrow> \<Gamma> \<turnstile> Lam [x].t : T1\<rightarrow>T2"
+| t_App[intro]:   "\<lbrakk>\<Gamma> \<turnstile> e\<^isub>1 : T\<^isub>1\<rightarrow>T\<^isub>2; \<Gamma> \<turnstile> e\<^isub>2 : T\<^isub>1\<rbrakk>\<Longrightarrow> \<Gamma> \<turnstile> App e\<^isub>1 e\<^isub>2 : T\<^isub>2"
+| t_Lam[intro]:   "\<lbrakk>x\<sharp>\<Gamma>; (x,T\<^isub>1)#\<Gamma> \<turnstile> t : T\<^isub>2\<rbrakk> \<Longrightarrow> \<Gamma> \<turnstile> Lam [x].t : T\<^isub>1\<rightarrow>T\<^isub>2"
 | t_Const[intro]: "valid \<Gamma> \<Longrightarrow> \<Gamma> \<turnstile> Const n : TBase"
 | t_Unit[intro]:  "valid \<Gamma> \<Longrightarrow> \<Gamma> \<turnstile> Unit : TUnit"
+(*>*)
+
+text {* 
+\begin{figure}
+\begin{center}
+\isastyle %smaller fonts
+@{thm[mode=Rule] t_Var[no_vars]}{\sc{t\_Var}}\qquad
+@{thm[mode=Rule] t_App[no_vars]}{\sc{t\_App}}\\
+@{thm[mode=Rule] t_Lam[no_vars]}{\sc{t\_Lam}}\\
+@{thm[mode=Rule] t_Const[no_vars]}{\sc{t\_Const}} \qquad
+@{thm[mode=Rule] t_Unit[no_vars]}{\sc{t\_Unit}}
+\end{center}
+\caption{Typing rules\label{typing}}
+\end{figure}
+*}
 
 lemma typing_valid:
   assumes "\<Gamma> \<turnstile> t : T"
   shows "valid \<Gamma>"
-  using assms
-  by (induct) (auto)
- 
-lemma typing_eqvt[eqvt]:
-  fixes pi::"name prm"
-  assumes "\<Gamma> \<turnstile> t : T"
-  shows "(pi\<bullet>\<Gamma>) \<turnstile> (pi\<bullet>t) : (pi\<bullet>T)"
-  using assms
-  apply(induct)
-  apply(auto simp add: fresh_bij set_eqvt valid_eqvt) 
-  apply(rule t_Var)
-  apply(drule valid_eqvt)
-  apply(assumption)
-  apply(drule in_eqvt)
-  apply(simp add: set_eqvt)
-  done
+  using assms by (induct)(auto)
 
-text {* Inversion lemmas for the typing judgment *}
+nominal_inductive typing
+
+text {* 
+\subsubsection{Inversion lemmas for the typing relation}
+
+We generate some inversion lemmas for 
+the typing judgment and add them as elimination rules for the automatic tactics.
+During the generation of these lemmas, we need the injectivity properties of the constructor of the nominal datatypes. These are not added by default in the set of simplification rules to prevent unwanted simplifications in the rest of the development. In the future, the \texttt{inductive\_cases} will be reworked to allow to use its own set of rules instead of the whole 'simpset'.
+*}
 
 declare trm.inject [simp add]
 declare ty.inject  [simp add]
@@ -157,16 +266,21 @@ inductive_cases2  t_Unit_elim_auto[elim]: "\<Gamma> \<turnstile> Unit : TUnit"
 declare trm.inject [simp del]
 declare ty.inject [simp del]
 
+text {* 
+\subsubsection{Strong induction principle}
+
+Now, we define a strong induction principle. This induction principle allow us to avoid some terms during the induction. The bound variable The avoided terms ($c$)  *}
+
 lemma typing_induct_strong
   [consumes 1, case_names t_Var t_App t_Lam t_Const t_Unit]:
     fixes  P::"'a::fs_name \<Rightarrow> (name\<times>ty) list \<Rightarrow> trm \<Rightarrow> ty \<Rightarrow>bool"
     and    x :: "'a::fs_name"
     assumes a: "\<Gamma> \<turnstile> e : T"
     and a1: "\<And>\<Gamma> x T c. \<lbrakk>valid \<Gamma>; (x,T)\<in>set \<Gamma>\<rbrakk> \<Longrightarrow> P c \<Gamma> (Var x) T"
-    and a2: "\<And>\<Gamma> e1 T1 T2 e2 c. \<lbrakk>\<And>c. P c \<Gamma> e1 (T1\<rightarrow>T2); \<And>c. P c \<Gamma> e2 T1\<rbrakk> 
-             \<Longrightarrow> P c \<Gamma> (App e1 e2) T2"
-    and a3: "\<And>x \<Gamma> T1 t T2 c.\<lbrakk>x\<sharp>(\<Gamma>,c); \<And>c. P c ((x,T1)#\<Gamma>) t T2\<rbrakk>
-             \<Longrightarrow> P c \<Gamma> (Lam [x].t) (T1\<rightarrow>T2)"
+    and a2: "\<And>\<Gamma> e\<^isub>1 T\<^isub>1 T\<^isub>2 e\<^isub>2 c. \<lbrakk>\<And>c. P c \<Gamma> e\<^isub>1 (T\<^isub>1\<rightarrow>T\<^isub>2); \<And>c. P c \<Gamma> e\<^isub>2 T\<^isub>1\<rbrakk> 
+             \<Longrightarrow> P c \<Gamma> (App e\<^isub>1 e\<^isub>2) T\<^isub>2"
+    and a3: "\<And>x \<Gamma> T\<^isub>1 t T\<^isub>2 c.\<lbrakk>x\<sharp>(\<Gamma>,c); \<And>c. P c ((x,T\<^isub>1)#\<Gamma>) t T\<^isub>2\<rbrakk>
+             \<Longrightarrow> P c \<Gamma> (Lam [x].t) (T\<^isub>1\<rightarrow>T\<^isub>2)"
     and a4: "\<And>\<Gamma> n c. valid \<Gamma> \<Longrightarrow> P c \<Gamma> (Const n) TBase"
     and a5: "\<And>\<Gamma> c. valid \<Gamma> \<Longrightarrow> P c \<Gamma> Unit TUnit"
     shows "P c \<Gamma> e T"
@@ -179,30 +293,30 @@ proof -
     moreover
     have "(x,T)\<in>set \<Gamma>" by fact
     then have "pi\<bullet>(x,T)\<in>pi\<bullet>(set \<Gamma>)" by (simp only: pt_set_bij[OF pt_name_inst, OF at_name_inst])  
-    then have "(pi\<bullet>x,T)\<in>set (pi\<bullet>\<Gamma>)" by (simp add: set_eqvt)
+    then have "(pi\<bullet>x,T)\<in>set (pi\<bullet>\<Gamma>)" by (simp add: eqvt)
     ultimately show "P c (pi\<bullet>\<Gamma>) (pi\<bullet>(Var x)) (pi\<bullet>T)" using a1 by simp
   next
-    case (t_App \<Gamma> e1 T1 T2 e2 pi c)
-    thus "P c (pi\<bullet>\<Gamma>) (pi\<bullet>(App e1 e2)) (pi\<bullet>T2)" using a2 
+    case (t_App \<Gamma> e\<^isub>1 T\<^isub>1 T\<^isub>2 e\<^isub>2 pi c)
+    thus "P c (pi\<bullet>\<Gamma>) (pi\<bullet>(App e\<^isub>1 e\<^isub>2)) (pi\<bullet>T\<^isub>2)" using a2 
       by (simp only: eqvt) (blast)
   next
-    case (t_Lam x \<Gamma> T1 t T2 pi c)
+    case (t_Lam x \<Gamma> T\<^isub>1 t T\<^isub>2 pi c)
     obtain y::"name" where fs: "y\<sharp>(pi\<bullet>x,pi\<bullet>\<Gamma>,pi\<bullet>t,c)" by (erule exists_fresh[OF fs_name1])
     let ?sw = "[(pi\<bullet>x,y)]"
     let ?pi' = "?sw@pi"
     have f0: "x\<sharp>\<Gamma>" by fact
     have f1: "(pi\<bullet>x)\<sharp>(pi\<bullet>\<Gamma>)" using f0 by (simp add: fresh_bij)
     have f2: "y\<sharp>?pi'\<bullet>\<Gamma>" by (auto simp add: pt_name2 fresh_left calc_atm perm_pi_simp)
-      have ih1: "\<And>c. P c (?pi'\<bullet>((x,T1)#\<Gamma>)) (?pi'\<bullet>t) (?pi'\<bullet>T2)" by fact
-    then have "P c (?pi'\<bullet>\<Gamma>) (Lam [y].(?pi'\<bullet>t)) (T1\<rightarrow>T2)" using fs f2 a3
+      have ih1: "\<And>c. P c (?pi'\<bullet>((x,T\<^isub>1)#\<Gamma>)) (?pi'\<bullet>t) (?pi'\<bullet>T\<^isub>2)" by fact
+    then have "P c (?pi'\<bullet>\<Gamma>) (Lam [y].(?pi'\<bullet>t)) (T\<^isub>1\<rightarrow>T\<^isub>2)" using fs f2 a3
       by (simp add: calc_atm)
-    then have "P c (?sw\<bullet>pi\<bullet>\<Gamma>) (?sw\<bullet>(Lam [(pi\<bullet>x)].(pi\<bullet>t))) (T1\<rightarrow>T2)" 
+    then have "P c (?sw\<bullet>pi\<bullet>\<Gamma>) (?sw\<bullet>(Lam [(pi\<bullet>x)].(pi\<bullet>t))) (T\<^isub>1\<rightarrow>T\<^isub>2)" 
       by (simp del: append_Cons add: calc_atm pt_name2)
     moreover have "(?sw\<bullet>pi\<bullet>\<Gamma>) = (pi\<bullet>\<Gamma>)"
       by (rule perm_fresh_fresh) (simp_all add: fs f1)
     moreover have "(?sw\<bullet>(Lam [(pi\<bullet>x)].(pi\<bullet>t))) = Lam [(pi\<bullet>x)].(pi\<bullet>t)"
       by (rule perm_fresh_fresh) (simp_all add: fs f1 fresh_atm abs_fresh)
-    ultimately show "P c (pi\<bullet>\<Gamma>) (pi\<bullet>(Lam [x].t)) (pi\<bullet>T1\<rightarrow>T2)" by simp
+    ultimately show "P c (pi\<bullet>\<Gamma>) (pi\<bullet>(Lam [x].t)) (pi\<bullet>T\<^isub>1\<rightarrow>T\<^isub>2)" by simp
   next
     case (t_Const \<Gamma> n pi c)
     thus "P c (pi\<bullet>\<Gamma>) (pi\<bullet>(Const n)) (pi\<bullet>TBase)" using a4 by (simp, blast intro: valid_eqvt)
@@ -214,7 +328,13 @@ proof -
   then show "P c \<Gamma> e T" by simp
 qed
 
-text {* capture-avoiding substitution *}
+text {* 
+\subsection{Capture-avoiding substitutions}
+
+In this section we define parallel substitution. The usual substitution will be derived as a special case of parallel substitution. But first we define a function to lookup for the term corresponding to a type in an association list. Note that if the term does not appear in the list then we return a variable of that name.\\
+Should we return Some or None and put that in a library ?
+ *}
+
 
 fun
   lookup :: "(name\<times>trm) list \<Rightarrow> name \<Rightarrow> trm"   
@@ -222,18 +342,17 @@ where
   "lookup [] X        = Var X"
   "lookup ((Y,T)#\<theta>) X = (if X=Y then T else lookup \<theta> X)"
 
-lemma lookup_eqvt:
+lemma lookup_eqvt[eqvt]:
   fixes pi::"name prm"
   and   \<theta>::"(name\<times>trm) list"
   and   X::"name"
   shows "pi\<bullet>(lookup \<theta> X) = lookup (pi\<bullet>\<theta>) (pi\<bullet>X)"
-by (induct \<theta>)
-   (auto simp add: perm_bij)
+by (induct \<theta>) (auto simp add: perm_bij)
 
 lemma lookup_fresh:
   fixes z::"name"
   assumes "z\<sharp>\<theta>" "z\<sharp>x"
-  shows "z \<sharp>lookup \<theta> x"
+  shows "z\<sharp> lookup \<theta> x"
 using assms 
 by (induct rule: lookup.induct) (auto simp add: fresh_list_cons)
 
@@ -244,22 +363,29 @@ using assms
 by (induct rule: lookup.induct)
    (auto simp add: fresh_list_cons fresh_prod fresh_atm)
 
+text {* \subsubsection{Parallel substitution} *}
+
 consts
   psubst :: "(name\<times>trm) list \<Rightarrow> trm \<Rightarrow> trm"  ("_<_>" [60,100] 100)
  
 nominal_primrec
   "\<theta><(Var x)> = (lookup \<theta> x)"
-  "\<theta><(App t1 t2)> = App (\<theta><t1>) (\<theta><t2>)"
+  "\<theta><(App t\<^isub>1 t\<^isub>2)> = App (\<theta><t\<^isub>1>) (\<theta><t\<^isub>2>)"
   "x\<sharp>\<theta> \<Longrightarrow> \<theta><(Lam [x].t)> = Lam [x].(\<theta><t>)"
   "\<theta><(Const n)> = Const n"
   "\<theta><(Unit)> = Unit"
-apply(finite_guess add: fs_name1 lookup_eqvt)+
-apply(perm_full_simp)
-apply(simp add: fs_name1)
+apply(finite_guess)+
 apply(rule TrueI)+
 apply(simp add: abs_fresh)+
-apply(fresh_guess add: fs_name1 lookup_eqvt)+
+apply(fresh_guess)+
 done
+
+
+text {* \subsubsection{Substitution} 
+
+The substitution function is defined just as a special case of parallel substitution. 
+
+*}
 
 abbreviation 
  subst :: "trm \<Rightarrow> name \<Rightarrow> trm \<Rightarrow> trm" ("_[_::=_]" [100,100,100] 100)
@@ -268,7 +394,7 @@ where
 
 lemma subst[simp]:
   shows "(Var x)[y::=t'] = (if x=y then t' else (Var x))"
-  and   "(App t1 t2)[y::=t'] = App (t1[y::=t']) (t2[y::=t'])"
+  and   "(App t\<^isub>1 t\<^isub>2)[y::=t'] = App (t\<^isub>1[y::=t']) (t\<^isub>2[y::=t'])"
   and   "x\<sharp>(y,t') \<Longrightarrow> (Lam [x].t)[y::=t'] = Lam [x].(t[y::=t'])"
   and   "Const n[y::=t'] = Const n"
   and   "Unit [y::=t'] = Unit"
@@ -281,13 +407,15 @@ lemma subst_eqvt[eqvt]:
   by (nominal_induct t avoiding: x t' rule: trm.induct)
      (perm_simp add: fresh_bij)+
 
+text {* \subsubsection{Lemmas about freshness and substitutions} *}
+
 lemma subst_rename: 
   fixes c::"name"
   and   t1::"trm"
-  assumes a: "c\<sharp>t1"
-  shows "t1[a::=t2] = ([(c,a)]\<bullet>t1)[c::=t2]"
+  assumes a: "c\<sharp>t\<^isub>1"
+  shows "t\<^isub>1[a::=t\<^isub>2] = ([(c,a)]\<bullet>t\<^isub>1)[c::=t\<^isub>2]"
   using a
-  apply(nominal_induct t1 avoiding: a c t2 rule: trm.induct)
+  apply(nominal_induct t\<^isub>1 avoiding: a c t\<^isub>2 rule: trm.induct)
   apply(simp add: trm.inject calc_atm fresh_atm abs_fresh perm_nat_def)+
   done
 
@@ -304,28 +432,28 @@ lemma fresh_subst'':
   fixes z::"name"
   and   t1::"trm"
   and   t2::"trm"
-  assumes "z\<sharp>t2"
-  shows "z\<sharp>t1[z::=t2]"
+  assumes "z\<sharp>t\<^isub>2"
+  shows "z\<sharp>t\<^isub>1[z::=t\<^isub>2]"
 using assms 
-by (nominal_induct t1 avoiding: t2 z rule: trm.induct)
+by (nominal_induct t\<^isub>1 avoiding: t\<^isub>2 z rule: trm.induct)
    (auto simp add: abs_fresh fresh_nat fresh_atm)
 
 lemma fresh_subst':
   fixes z::"name"
   and   t1::"trm"
   and   t2::"trm"
-  assumes "z\<sharp>[y].t1" "z\<sharp>t2"
-  shows "z\<sharp>t1[y::=t2]"
+  assumes "z\<sharp>[y].t\<^isub>1" "z\<sharp>t\<^isub>2"
+  shows "z\<sharp>t\<^isub>1[y::=t\<^isub>2]"
 using assms 
-by (nominal_induct t1 avoiding: y t2 z rule: trm.induct)
+by (nominal_induct t\<^isub>1 avoiding: y t\<^isub>2 z rule: trm.induct)
    (auto simp add: abs_fresh fresh_nat fresh_atm)
 
 lemma fresh_subst:
   fixes z::"name"
   and   t1::"trm"
   and   t2::"trm"
-  assumes "z\<sharp>t1" "z\<sharp>t2"
-  shows "z\<sharp>t1[y::=t2]"
+  assumes "z\<sharp>t\<^isub>1" "z\<sharp>t\<^isub>2"
+  shows "z\<sharp>t\<^isub>1[y::=t\<^isub>2]"
 using assms fresh_subst'
 by (auto simp add: abs_fresh) 
 
@@ -346,415 +474,6 @@ proof (nominal_induct t avoiding: x u \<theta> rule: trm.induct)
   ultimately show "(x,u)#\<theta><Lam [y].t> = \<theta><Lam [y].t>" by auto
 qed (auto simp add: fresh_atm abs_fresh)
 
-text {* Equivalence (defined) *}
-
-inductive2
-  equiv_def :: "(name\<times>ty) list\<Rightarrow>trm\<Rightarrow>trm\<Rightarrow>ty\<Rightarrow>bool" ("_ \<turnstile> _ == _ : _" [60,60] 60) 
-where
-  Q_Refl[intro]:  "\<Gamma> \<turnstile> t : T \<Longrightarrow> \<Gamma> \<turnstile> t == t : T"
-| Q_Symm[intro]:  "\<Gamma> \<turnstile> t == s : T \<Longrightarrow> \<Gamma> \<turnstile> s == t : T"
-| Q_Trans[intro]: "\<lbrakk>\<Gamma> \<turnstile> s == t : T; \<Gamma> \<turnstile> t == u : T\<rbrakk> \<Longrightarrow>  \<Gamma> \<turnstile> s == u : T"
-| Q_Abs[intro]:   "\<lbrakk>x\<sharp>\<Gamma>; (x,T1)#\<Gamma> \<turnstile> s2 == t2 : T2\<rbrakk> \<Longrightarrow> \<Gamma> \<turnstile> Lam [x]. s2 ==  Lam [x]. t2 : T1 \<rightarrow> T2"
-| Q_App[intro]:   "\<lbrakk>\<Gamma> \<turnstile> s1 == t1 : T1 \<rightarrow> T2 ; \<Gamma> \<turnstile> s2 == t2 : T1\<rbrakk> \<Longrightarrow>  \<Gamma> \<turnstile> App s1 s2 == App t1 t2 : T2"
-| Q_Beta[intro]:  "\<lbrakk>x\<sharp>(\<Gamma>,s2,t2); (x,T1)#\<Gamma> \<turnstile> s12 == t12 : T2 ; \<Gamma> \<turnstile> s2 == t2 : T1\<rbrakk> 
-                   \<Longrightarrow>  \<Gamma> \<turnstile> App (Lam [x]. s12) s2 ==  t12[x::=t2] : T2"
-| Q_Ext[intro]:   "\<lbrakk>x\<sharp>(\<Gamma>,s,t); (x,T1)#\<Gamma> \<turnstile> App s (Var x) == App t (Var x) : T2\<rbrakk> 
-                   \<Longrightarrow> \<Gamma> \<turnstile> s == t : T1 \<rightarrow> T2"
-
-lemma equiv_def_valid:
-  assumes "\<Gamma> \<turnstile> t == s : T"
-  shows "valid \<Gamma>"
-using assms by (induct,auto elim:typing_valid)
-
-lemma equiv_def_eqvt[eqvt]:
-  fixes pi::"name prm"
-  assumes a: "\<Gamma> \<turnstile> s == t : T"
-  shows "(pi\<bullet>\<Gamma>) \<turnstile> (pi\<bullet>s) == (pi\<bullet>t) : (pi\<bullet>T)"
-using a
-apply(induct)
-apply(auto intro: typing_eqvt valid_eqvt simp add: fresh_bij subst_eqvt simp del: perm_ty)
-apply(rule_tac x="pi\<bullet>x" in Q_Ext)
-apply(simp add: fresh_bij)+
-done
-
-lemma equiv_def_strong_induct
-  [consumes 1, case_names Q_Refl Q_Symm Q_Trans Q_Abs Q_App Q_Beta Q_Ext]:
-  fixes c::"'a::fs_name"
-  assumes a0: "\<Gamma> \<turnstile> s == t : T" 
-  and     a1: "\<And>\<Gamma> t T c.  \<Gamma> \<turnstile> t : T  \<Longrightarrow> P c \<Gamma> t t T"
-  and     a2: "\<And>\<Gamma> t s T c. \<lbrakk>\<And>d. P d \<Gamma> t s T\<rbrakk> \<Longrightarrow>  P c \<Gamma> s t T"
-  and     a3: "\<And>\<Gamma> s t T u c. \<lbrakk>\<And>d. P d \<Gamma> s t T; \<And>d. P d \<Gamma> t u T\<rbrakk> 
-               \<Longrightarrow> P c \<Gamma> s u T"
-  and     a4: "\<And>x \<Gamma> T1 s2 t2 T2 c. \<lbrakk>x\<sharp>\<Gamma>; x\<sharp>c; \<And>d. P d ((x,T1)#\<Gamma>) s2 t2 T2\<rbrakk>
-               \<Longrightarrow> P c \<Gamma> (Lam [x].s2) (Lam [x].t2) (T1\<rightarrow>T2)"
-  and     a5: "\<And>\<Gamma> s1 t1 T1 T2 s2 t2 c. \<lbrakk>\<And>d. P d \<Gamma> s1 t1 (T1\<rightarrow>T2); \<And>d. P d \<Gamma> s2 t2 T1\<rbrakk> 
-               \<Longrightarrow> P c \<Gamma> (App s1 s2) (App t1 t2) T2"
-  and     a6: "\<And>x \<Gamma> T1 s12 t12 T2 s2 t2 c.
-               \<lbrakk>x\<sharp>(\<Gamma>,s2,t2); x\<sharp>c; \<And>d. P d ((x,T1)#\<Gamma>) s12 t12 T2; \<And>d. P d \<Gamma> s2 t2 T1\<rbrakk> 
-               \<Longrightarrow> P c \<Gamma> (App (Lam [x].s12) s2) (t12[x::=t2]) T2"
-  and     a7: "\<And>x \<Gamma> s t T1 T2 c.
-               \<lbrakk>x\<sharp>(\<Gamma>,s,t); \<And>d. P d ((x,T1)#\<Gamma>) (App s (Var x)) (App t (Var x)) T2\<rbrakk>
-               \<Longrightarrow> P c \<Gamma> s t (T1\<rightarrow>T2)"
- shows "P c \<Gamma>  s t T"
-proof -
-  from a0 have "\<And>(pi::name prm) c. P c (pi\<bullet>\<Gamma>) (pi\<bullet>s) (pi\<bullet>t) (pi\<bullet>T)" 
-    proof(induct)
-      case (Q_Refl \<Gamma> t T pi c)
-      then show "P c (pi\<bullet>\<Gamma>) (pi\<bullet>t) (pi\<bullet>t) (pi\<bullet>T)" using a1 by (simp only: eqvt)
-    next
-      case (Q_Symm \<Gamma> t s T pi c)
-      then show "P c (pi\<bullet>\<Gamma>) (pi\<bullet>s) (pi\<bullet>t) (pi\<bullet>T)" using a2 by (simp only: equiv_def_eqvt)
-    next
-      case (Q_Trans \<Gamma> s t T u pi c)
-      then show " P c (pi\<bullet>\<Gamma>) (pi\<bullet>s) (pi\<bullet>u) (pi\<bullet>T)" using a3 by (blast intro: equiv_def_eqvt)
-    next
-      case (Q_App \<Gamma> s1 t1 T1 T2 s2 t2 pi c)
-      then show "P c (pi\<bullet>\<Gamma>) (pi\<bullet>App s1 s2) (pi\<bullet>App t1 t2) (pi\<bullet>T2)" using a5 
-	by (simp only: eqvt) (blast)
-    next
-      case (Q_Ext x \<Gamma> s t T1 T2 pi c)
-      then show "P c (pi\<bullet>\<Gamma>) (pi\<bullet>s) (pi\<bullet>t) (pi\<bullet>T1\<rightarrow>T2)"  
-	by (auto intro!: a7 simp add: fresh_bij)
-    next
-      case (Q_Abs x \<Gamma> T1 s2 t2 T2 pi c)
-      obtain y::"name" where fs: "y\<sharp>(pi\<bullet>x,pi\<bullet>s2,pi\<bullet>t2,pi\<bullet>\<Gamma>,c)" by (rule exists_fresh[OF fs_name1])
-      let ?sw="[(pi\<bullet>x,y)]"
-      let ?pi'="?sw@pi"
-      have f1: "x\<sharp>\<Gamma>" by fact
-      have f2: "(pi\<bullet>x)\<sharp>(pi\<bullet>\<Gamma>)" using f1 by (simp add: fresh_bij)
-      have f3: "y\<sharp>?pi'\<bullet>\<Gamma>" using f1 by (auto simp add: pt_name2 fresh_left calc_atm perm_pi_simp)
-      have ih1: "\<And>c. P c (?pi'\<bullet>((x,T1)#\<Gamma>)) (?pi'\<bullet>s2) (?pi'\<bullet>t2) (?pi'\<bullet>T2)" by fact
-      then have "\<And>c. P c ((y,T1)#(?pi'\<bullet>\<Gamma>)) (?pi'\<bullet>s2) (?pi'\<bullet>t2) T2" by (simp add: calc_atm)
-      then have "P c  (?pi'\<bullet>\<Gamma>) (?pi'\<bullet>Lam [x].s2) (?pi'\<bullet>Lam [x].t2) (T1\<rightarrow>T2)" using a4 f3 fs
-	by (simp add: calc_atm)
-      then have "P c (?sw\<bullet>pi\<bullet>\<Gamma>) (?sw\<bullet>Lam [(pi\<bullet>x)].(pi\<bullet>s2)) (?sw\<bullet>Lam [(pi\<bullet>x)].(pi\<bullet>t2)) (T1\<rightarrow>T2)" 
-	by (simp del: append_Cons add: calc_atm pt_name2)
-      moreover have "(?sw\<bullet>(pi\<bullet>\<Gamma>)) = (pi\<bullet>\<Gamma>)" 
-	by (rule perm_fresh_fresh) (simp_all add: fs f2)
-      moreover have "(?sw\<bullet>(Lam [(pi\<bullet>x)].(pi\<bullet>s2))) = Lam [(pi\<bullet>x)].(pi\<bullet>s2)" 
-	by (rule perm_fresh_fresh) (simp_all add: fs f2 abs_fresh)
-      moreover have "(?sw\<bullet>(Lam [(pi\<bullet>x)].(pi\<bullet>t2))) = Lam [(pi\<bullet>x)].(pi\<bullet>t2)" 
-	by (rule perm_fresh_fresh) (simp_all add: fs f2 abs_fresh)
-      ultimately have "P c (pi\<bullet>\<Gamma>) (Lam [(pi\<bullet>x)].(pi\<bullet>s2)) (Lam [(pi\<bullet>x)].(pi\<bullet>t2)) (T1\<rightarrow>T2)" by simp
-      then show  "P c (pi\<bullet>\<Gamma>) (pi\<bullet>Lam [x].s2) (pi\<bullet>Lam [x].t2) (pi\<bullet>T1\<rightarrow>T2)" by simp 
-    next 
-      case (Q_Beta x \<Gamma> s2 t2 T1 s12 t12 T2 pi c) 
-      obtain y::"name" where fs: "y\<sharp>(pi\<bullet>x,pi\<bullet>s12,pi\<bullet>t12,pi\<bullet>s2,pi\<bullet>t2,pi\<bullet>\<Gamma>,c)" 
-	by (rule exists_fresh[OF fs_name1])
-      let ?sw="[(pi\<bullet>x,y)]"
-      let ?pi'="?sw@pi"
-      have f1: "x\<sharp>(\<Gamma>,s2,t2)" by fact 
-      have f2: "(pi\<bullet>x)\<sharp>(pi\<bullet>(\<Gamma>,s2,t2))" using f1 by (simp add: fresh_bij)
-      have f3: "y\<sharp>(?pi'\<bullet>(\<Gamma>,s2,t2))" using f1 
-	by (auto simp add: pt_name2 fresh_left calc_atm perm_pi_simp fresh_prod)
-      have ih1: "\<And>c. P c (?pi'\<bullet>((x,T1)#\<Gamma>)) (?pi'\<bullet>s12) (?pi'\<bullet>t12) (?pi'\<bullet>T2)" by fact
-      then have "\<And>c. P c ((y,T1)#(?pi'\<bullet>\<Gamma>)) (?pi'\<bullet>s12) (?pi'\<bullet>t12) (?pi'\<bullet>T2)" by (simp add: calc_atm)
-      moreover
-      have ih2: "\<And>c. P c (?pi'\<bullet>\<Gamma>) (?pi'\<bullet>s2) (?pi'\<bullet>t2) (?pi'\<bullet>T1)" by fact
-      ultimately have "P c  (?pi'\<bullet>\<Gamma>) (?pi'\<bullet>(App (Lam [x].s12) s2)) (?pi'\<bullet>(t12[x::=t2])) (?pi'\<bullet>T2)" 
-	using a6 f3 fs by (force simp add: subst_eqvt calc_atm del: perm_ty)
-      then have "P c (?sw\<bullet>pi\<bullet>\<Gamma>) (?sw\<bullet>(App (Lam [(pi\<bullet>x)].(pi\<bullet>s12)) (pi\<bullet>s2))) 
-	(?sw\<bullet>((pi\<bullet>t12)[(pi\<bullet>x)::=(pi\<bullet>t2)])) T2" 
-	by (simp del: append_Cons add: calc_atm pt_name2 subst_eqvt)
-      moreover have "(?sw\<bullet>(pi\<bullet>\<Gamma>)) = (pi\<bullet>\<Gamma>)" 
-	by (rule perm_fresh_fresh) (simp_all add: fs[simplified] f2[simplified])
-      moreover have "(?sw\<bullet>(App (Lam [(pi\<bullet>x)].(pi\<bullet>s12)) (pi\<bullet>s2))) = App (Lam [(pi\<bullet>x)].(pi\<bullet>s12)) (pi\<bullet>s2)" 
-	by (rule perm_fresh_fresh) (simp_all add: fs[simplified] f2[simplified] abs_fresh)
-      moreover have "(?sw\<bullet>((pi\<bullet>t12)[(pi\<bullet>x)::=(pi\<bullet>t2)])) = ((pi\<bullet>t12)[(pi\<bullet>x)::=(pi\<bullet>t2)])" 
-	by (rule perm_fresh_fresh) 
-	   (simp_all add: fs[simplified] f2[simplified] fresh_subst fresh_subst'')
-      ultimately have "P c (pi\<bullet>\<Gamma>) (App (Lam [(pi\<bullet>x)].(pi\<bullet>s12)) (pi\<bullet>s2)) ((pi\<bullet>t12)[(pi\<bullet>x)::=(pi\<bullet>t2)]) T2"
-	by simp
-      then show "P c (pi\<bullet>\<Gamma>) (pi\<bullet>App (Lam [x].s12) s2) (pi\<bullet>t12[x::=t2]) (pi\<bullet>T2)" by (simp add: subst_eqvt)
-    qed
-  then have "P c (([]::name prm)\<bullet>\<Gamma>) (([]::name prm)\<bullet>s) (([]::name prm)\<bullet>t) (([]::name prm)\<bullet>T)" by blast
-  then show "P c \<Gamma> s t T" by simp
-qed
-
-text {* Weak head reduction *}
-
-inductive2
-  whr_def :: "trm\<Rightarrow>trm\<Rightarrow>bool" ("_ \<leadsto> _" [80,80] 80) 
-where
-  QAR_Beta[intro]: "App (Lam [x]. t12) t2 \<leadsto> t12[x::=t2]"
-| QAR_App[intro]: "t1 \<leadsto> t1' \<Longrightarrow> App t1 t2 \<leadsto> App t1' t2"
-
-declare trm.inject  [simp add]
-declare ty.inject  [simp add]
-
-inductive_cases2 whr_Gen[elim]: "t \<leadsto> t'"
-inductive_cases2 whr_Lam[elim]: "Lam [x].t \<leadsto> t'"
-inductive_cases2 whr_App_Lam[elim]: "App (Lam [x].t12) t2 \<leadsto> t"
-inductive_cases2 whr_Var[elim]: "Var x \<leadsto> t"
-inductive_cases2 whr_Const[elim]: "Const n \<leadsto> t"
-inductive_cases2 whr_App[elim]: "App p q \<leadsto> t"
-inductive_cases2 whr_Const_Right[elim]: "t \<leadsto> Const n"
-inductive_cases2 whr_Var_Right[elim]: "t \<leadsto> Var x"
-inductive_cases2 whr_App_Right[elim]: "t \<leadsto> App p q"
-
-declare trm.inject  [simp del]
-declare ty.inject  [simp del]
-
-text {* Weak head normalization *}
-
-abbreviation 
- nf :: "trm \<Rightarrow> bool" ("_ \<leadsto>|" [100] 100)
-where
-  "t\<leadsto>|  \<equiv> \<not>(\<exists> u. t \<leadsto> u)" 
-
-inductive2
-  whn_def :: "trm\<Rightarrow>trm\<Rightarrow>bool" ("_ \<Down> _" [80,80] 80) 
-where
-  QAN_Reduce[intro]: "\<lbrakk>s \<leadsto> t; t \<Down> u\<rbrakk> \<Longrightarrow> s \<Down> u"
-| QAN_Normal[intro]: "t\<leadsto>|  \<Longrightarrow> t \<Down> t"
-
-lemma whr_eqvt:
-  fixes pi::"name prm"
-  assumes a: "t \<leadsto> t'"
-  shows "(pi\<bullet>t) \<leadsto> (pi\<bullet>t')"
-using a
-by (induct) (auto simp add: subst_eqvt fresh_bij)
-
-lemma whn_eqvt[eqvt]:
-  fixes pi::"name prm"
-  assumes a: "t \<Down> t'"
-  shows "(pi\<bullet>t) \<Down> (pi\<bullet>t')"
-using a
-apply(induct)
-apply(rule QAN_Reduce)
-apply(rule whr_eqvt)
-apply(assumption)+
-apply(rule QAN_Normal)
-apply(auto)
-apply(drule_tac pi="rev pi" in whr_eqvt)
-apply(perm_simp)
-done
-
-text {* Algorithmic term equivalence and algorithmic path equivalence *}
-
-inductive2
-  alg_equiv :: "(name\<times>ty) list\<Rightarrow>trm\<Rightarrow>trm\<Rightarrow>ty\<Rightarrow>bool" ("_ \<turnstile> _ <=> _ : _" [60,60] 60) 
-and
-  alg_path_equiv :: "(name\<times>ty) list\<Rightarrow>trm\<Rightarrow>trm\<Rightarrow>ty\<Rightarrow>bool" ("_ \<turnstile> _ \<leftrightarrow> _ : _" [60,60] 60) 
-where
-  QAT_Base[intro]:  "\<lbrakk>s \<Down> p; t \<Down> q; \<Gamma> \<turnstile> p \<leftrightarrow> q : TBase \<rbrakk> \<Longrightarrow> \<Gamma> \<turnstile> s <=> t : TBase"
-| QAT_Arrow[intro]: "\<lbrakk>x\<sharp>\<Gamma>; x\<sharp>s; x\<sharp>t; (x,T1)#\<Gamma> \<turnstile> App s (Var x) <=> App t (Var x) : T2\<rbrakk> 
-                     \<Longrightarrow> \<Gamma> \<turnstile> s <=> t : T1 \<rightarrow> T2"
-| QAT_One[intro]:   "valid \<Gamma> \<Longrightarrow> \<Gamma> \<turnstile> s <=> t : TUnit"
-| QAP_Var[intro]:   "\<lbrakk>valid \<Gamma>;(x,T) \<in> set \<Gamma>\<rbrakk> \<Longrightarrow> \<Gamma> \<turnstile> Var x \<leftrightarrow> Var x : T"
-| QAP_App[intro]:   "\<lbrakk>\<Gamma> \<turnstile> p \<leftrightarrow> q : T1 \<rightarrow> T2; \<Gamma> \<turnstile> s <=> t : T1 \<rbrakk> \<Longrightarrow> \<Gamma> \<turnstile> App p s \<leftrightarrow> App q t : T2"
-| QAP_Const[intro]: "valid \<Gamma> \<Longrightarrow> \<Gamma> \<turnstile> Const n \<leftrightarrow> Const n : TBase"
-
-lemma alg_equiv_alg_path_equiv_eqvt[eqvt]:
-  fixes pi::"name prm"
-  shows "\<Gamma> \<turnstile> s <=> t : T \<Longrightarrow> (pi\<bullet>\<Gamma>) \<turnstile> (pi\<bullet>s) <=> (pi\<bullet>t) : (pi\<bullet>T)" 
-  and   "\<Gamma> \<turnstile> p \<leftrightarrow> q : T \<Longrightarrow> (pi\<bullet>\<Gamma>) \<turnstile> (pi\<bullet>p) \<leftrightarrow> (pi\<bullet>q) : (pi\<bullet>T)"
-apply(induct rule: alg_equiv_alg_path_equiv.inducts)
-apply(auto intro: whn_eqvt simp add: fresh_bij valid_eqvt)
-apply(rule_tac x="pi\<bullet>x" in  QAT_Arrow)
-apply(auto simp add: fresh_bij)
-apply(rule QAP_Var)
-apply(simp add: valid_eqvt)
-apply(simp add: pt_list_set_pi[OF pt_name_inst, symmetric])
-apply(perm_simp add: pt_set_bij1a[OF pt_name_inst, OF at_name_inst])
-done
-
-lemma alg_equiv_alg_path_equiv_strong_induct
-  [case_names QAT_Base QAT_Arrow QAT_One QAP_Var QAP_App QAP_Const]:
-  fixes c::"'a::fs_name"
-  assumes a1: "\<And>s p t q \<Gamma> c. \<lbrakk>s \<Down> p; t \<Down> q; \<Gamma> \<turnstile> p \<leftrightarrow> q : TBase; \<And>d. P2 d \<Gamma> p q TBase\<rbrakk> 
-               \<Longrightarrow> P1 c \<Gamma> s t TBase"
-  and     a2: "\<And>x \<Gamma> s t T1 T2 c.
-               \<lbrakk>x\<sharp>\<Gamma>; x\<sharp>s; x\<sharp>t; x\<sharp>c; (x,T1)#\<Gamma> \<turnstile> App s (Var x) <=> App t (Var x) : T2;
-               \<And>d. P1 d ((x,T1)#\<Gamma>) (App s (Var x)) (App t (Var x)) T2\<rbrakk>
-               \<Longrightarrow> P1 c \<Gamma> s t (T1\<rightarrow>T2)"
-  and     a3: "\<And>\<Gamma> s t c. valid \<Gamma> \<Longrightarrow> P1 c \<Gamma> s t TUnit"
-  and     a4: "\<And>\<Gamma> x T c. \<lbrakk>valid \<Gamma>; (x,T) \<in> set \<Gamma>\<rbrakk> \<Longrightarrow> P2 c \<Gamma> (Var x) (Var x) T"
-  and     a5: "\<And>\<Gamma> p q T1 T2 s t c.
-               \<lbrakk>\<Gamma> \<turnstile> p \<leftrightarrow> q : T1\<rightarrow>T2; \<And>d. P2 d \<Gamma> p q (T1\<rightarrow>T2); \<Gamma> \<turnstile> s <=> t : T1; \<And>d. P1 d \<Gamma> s t T1\<rbrakk>
-               \<Longrightarrow> P2 c \<Gamma> (App p s) (App q t) T2"
-  and     a6: "\<And>\<Gamma> n c. valid \<Gamma> \<Longrightarrow> P2 c \<Gamma> (Const n) (Const n) TBase"
-  shows "(\<Gamma> \<turnstile> s <=> t : T \<longrightarrow>P1 c \<Gamma> s t T) \<and> (\<Gamma>' \<turnstile> s' \<leftrightarrow> t' : T' \<longrightarrow> P2 c \<Gamma>' s' t' T')"
-proof -
-  have "(\<Gamma> \<turnstile> s <=> t : T \<longrightarrow> (\<forall>c (pi::name prm). P1 c (pi\<bullet>\<Gamma>) (pi\<bullet>s) (pi\<bullet>t) T)) \<and> 
-        (\<Gamma>' \<turnstile> s' \<leftrightarrow> t' : T' \<longrightarrow> (\<forall>c (pi::name prm). P2 c (pi\<bullet>\<Gamma>') (pi\<bullet>s') (pi\<bullet>t') T'))"
-  proof(induct rule: alg_equiv_alg_path_equiv.induct)
-    case (QAT_Base s q t p \<Gamma>)
-    then show "\<forall>c (pi::name prm). P1 c (pi\<bullet>\<Gamma>) (pi\<bullet>s) (pi\<bullet>t) TBase"
-      apply(auto)
-      apply(rule_tac p="pi\<bullet>q" and q="pi\<bullet>p" in  a1)
-      apply(simp_all add: whn_eqvt alg_equiv_alg_path_equiv_eqvt[simplified])
-      done
-  next
-    case (QAT_Arrow x \<Gamma> s t T1 T2)
-    show ?case
-    proof (rule allI, rule allI)
-      fix c::"'a::fs_name" and pi::"name prm"
-      obtain y::"name" where fs: "y\<sharp>(pi\<bullet>s,pi\<bullet>t,pi\<bullet>\<Gamma>,c)" by (rule exists_fresh[OF fs_name1])
-      let ?sw="[(pi\<bullet>x,y)]"
-      let ?pi'="?sw@pi"
-      have f0: "x\<sharp>\<Gamma>" "x\<sharp>s" "x\<sharp>t" by fact
-      then have f1: "x\<sharp>(\<Gamma>,s,t)" by simp
-      have f2: "(pi\<bullet>x)\<sharp>(pi\<bullet>(\<Gamma>,s,t))" using f1 by (simp add: fresh_bij)
-      have f3: "y\<sharp>?pi'\<bullet>(\<Gamma>,s,t)" using f1 
-	by (simp only: pt_name2 fresh_left, auto simp add: perm_pi_simp calc_atm)
-      then have f3': "y\<sharp>?pi'\<bullet>\<Gamma>" "y\<sharp>?pi'\<bullet>s" "y\<sharp>?pi'\<bullet>t" by (auto simp add: fresh_prod)
-      have pr1: "(x,T1)#\<Gamma> \<turnstile> App s (Var x) <=> App t (Var x) : T2" by fact
-      then have "(?pi'\<bullet>((x,T1)#\<Gamma>)) \<turnstile> (?pi'\<bullet>(App s (Var x))) <=> (?pi'\<bullet>(App t (Var x))) : (?pi'\<bullet>T2)" 
-	by (rule alg_equiv_alg_path_equiv_eqvt)
-      then have "(y,T1)#(?pi'\<bullet>\<Gamma>) \<turnstile> (App (?pi'\<bullet>s) (Var y)) <=> (App (?pi'\<bullet>t) (Var y)) : T2" 
-	by (simp add: calc_atm)
-      moreover    
-      have ih1: "\<forall>c (pi::name prm).  P1 c (pi\<bullet>((x,T1)#\<Gamma>)) (pi\<bullet>App s (Var x)) (pi\<bullet>App t (Var x)) T2"
-	by fact
-      then have "\<And>c.  P1 c (?pi'\<bullet>((x,T1)#\<Gamma>)) (?pi'\<bullet>App s (Var x)) (?pi'\<bullet>App t (Var x)) T2"
-	by auto
-      then have "\<And>c.  P1 c ((y,T1)#(?pi'\<bullet>\<Gamma>)) (App (?pi'\<bullet>s) (Var y)) (App (?pi'\<bullet>t) (Var y)) T2"
-	by (simp add: calc_atm)     
-      ultimately have "P1 c (?pi'\<bullet>\<Gamma>) (?pi'\<bullet>s) (?pi'\<bullet>t) (T1\<rightarrow>T2)" using a2 f3' fs by simp
-      then have "P1 c (?sw\<bullet>pi\<bullet>\<Gamma>) (?sw\<bullet>pi\<bullet>s) (?sw\<bullet>pi\<bullet>t) (T1\<rightarrow>T2)" 
-	by (simp del: append_Cons add: calc_atm pt_name2)
-      moreover have "(?sw\<bullet>(pi\<bullet>\<Gamma>)) = (pi\<bullet>\<Gamma>)" 
-	by (rule perm_fresh_fresh) (simp_all add: fs[simplified] f2[simplified])
-      moreover have "(?sw\<bullet>(pi\<bullet>s)) = (pi\<bullet>s)" 
-	by (rule perm_fresh_fresh) (simp_all add: fs[simplified] f2[simplified])
-      moreover have "(?sw\<bullet>(pi\<bullet>t)) = (pi\<bullet>t)" 
-	by (rule perm_fresh_fresh) (simp_all add: fs[simplified] f2[simplified])
-      ultimately show "P1 c (pi\<bullet>\<Gamma>) (pi\<bullet>s) (pi\<bullet>t) (T1\<rightarrow>T2)" by (simp)
-    qed
-  next
-    case (QAT_One \<Gamma> s t)
-    then show "\<forall>c (pi::name prm). P1 c (pi\<bullet>\<Gamma>) (pi\<bullet>s) (pi\<bullet>t) TUnit"
-      by (auto intro!: a3 simp add: valid_eqvt)
-  next
-    case (QAP_Var \<Gamma> x T)
-    then show "\<forall>c (pi::name prm). P2 c (pi \<bullet> \<Gamma>) (pi \<bullet> Var x) (pi \<bullet> Var x) T"
-      apply(auto intro!: a4 simp add: valid_eqvt)
-      apply(simp add: pt_list_set_pi[OF pt_name_inst, symmetric])
-      apply(perm_simp add: pt_set_bij1a[OF pt_name_inst, OF at_name_inst])
-      done
-  next
-    case (QAP_App \<Gamma> p q T1 T2 s t)
-    then show "\<forall>c (pi::name prm). P2 c (pi\<bullet>\<Gamma>) (pi\<bullet>App p s) (pi\<bullet>App q t) T2"
-      by (auto intro!: a5 simp add: alg_equiv_alg_path_equiv_eqvt[simplified])
-  next
-    case (QAP_Const \<Gamma> n)
-    then show "\<forall>c (pi::name prm). P2 c (pi\<bullet>\<Gamma>) (pi\<bullet>Const n) (pi\<bullet>Const n) TBase"
-      by (auto intro!: a6 simp add: valid_eqvt)
-  qed
-  then have "(\<Gamma> \<turnstile> s <=> t : T \<longrightarrow> P1 c (([]::name prm)\<bullet>\<Gamma>) (([]::name prm)\<bullet>s) (([]::name prm)\<bullet>t) T) \<and> 
-             (\<Gamma>' \<turnstile> s' \<leftrightarrow> t' : T' \<longrightarrow> P2 c (([]::name prm)\<bullet>\<Gamma>') (([]::name prm)\<bullet>s') (([]::name prm)\<bullet>t') T')"
-    by blast
-  then show ?thesis by simp
-qed
-
-(* post-processing of the strong induction principle proved above; *) 
-(* the code extracts the strong_inducts-version from strong_induct *)
-setup {*
-  PureThy.add_thmss
-    [(("alg_equiv_alg_path_equiv_strong_inducts",
-      ProjectRule.projects (ProofContext.init (the_context())) [1,2]
-        (thm "alg_equiv_alg_path_equiv_strong_induct")), [])] #> snd
-*}
-
-declare trm.inject  [simp add]
-declare ty.inject  [simp add]
-
-inductive_cases2 whn_inv_auto[elim]: "t \<Down> t'"
-
-inductive_cases2 alg_equiv_Base_inv_auto[elim]: "\<Gamma> \<turnstile> s<=>t : TBase"
-inductive_cases2 alg_equiv_Arrow_inv_auto[elim]: "\<Gamma> \<turnstile> s<=>t : T1 \<rightarrow> T2"
-
-inductive_cases2 alg_path_equiv_Base_inv_auto[elim]: "\<Gamma> \<turnstile> s\<leftrightarrow>t : TBase"
-inductive_cases2 alg_path_equiv_Unit_inv_auto[elim]: "\<Gamma> \<turnstile> s\<leftrightarrow>t : TUnit"
-inductive_cases2 alg_path_equiv_Arrow_inv_auto[elim]: "\<Gamma> \<turnstile> s\<leftrightarrow>t : T1 \<rightarrow> T2"
-
-inductive_cases2 alg_path_equiv_Var_left_inv_auto[elim]: "\<Gamma> \<turnstile> Var x \<leftrightarrow> t : T"
-inductive_cases2 alg_path_equiv_Var_left_inv_auto'[elim]: "\<Gamma> \<turnstile> Var x \<leftrightarrow> t : T'"
-inductive_cases2 alg_path_equiv_Var_right_inv_auto[elim]: "\<Gamma> \<turnstile> s \<leftrightarrow> Var x : T"
-inductive_cases2 alg_path_equiv_Var_right_inv_auto'[elim]: "\<Gamma> \<turnstile> s \<leftrightarrow> Var x : T'"
-inductive_cases2 alg_path_equiv_Const_left_inv_auto[elim]: "\<Gamma> \<turnstile> Const n \<leftrightarrow> t : T"
-inductive_cases2 alg_path_equiv_Const_right_inv_auto[elim]: "\<Gamma> \<turnstile> s \<leftrightarrow> Const n : T"
-inductive_cases2 alg_path_equiv_App_left_inv_auto[elim]: "\<Gamma> \<turnstile> App p s \<leftrightarrow> t : T"
-inductive_cases2 alg_path_equiv_App_right_inv_auto[elim]: "\<Gamma> \<turnstile> s \<leftrightarrow> App q t : T"
-inductive_cases2 alg_path_equiv_Lam_left_inv_auto[elim]: "\<Gamma> \<turnstile> Lam[x].s \<leftrightarrow> t : T"
-inductive_cases2 alg_path_equiv_Lam_right_inv_auto[elim]: "\<Gamma> \<turnstile> t \<leftrightarrow> Lam[x].s : T"
-
-declare trm.inject [simp del]
-declare ty.inject [simp del]
-
-text {* Subcontext. *}
-
-abbreviation
-  "sub" :: "(name\<times>ty) list \<Rightarrow> (name\<times>ty) list \<Rightarrow> bool" (" _ \<lless> _ " [55,55] 55)
-where
-  "\<Gamma>1 \<lless> \<Gamma>2 \<equiv> (\<forall>a \<sigma>. (a,\<sigma>)\<in>set \<Gamma>1 \<longrightarrow>  (a,\<sigma>)\<in>set \<Gamma>2) \<and> valid \<Gamma>2"
-
-lemma alg_equiv_valid:
-  shows  "\<Gamma> \<turnstile> s <=> t : T \<Longrightarrow> valid \<Gamma>" and  "\<Gamma> \<turnstile> s \<leftrightarrow> t : T \<Longrightarrow> valid \<Gamma>"
-by (induct rule : alg_equiv_alg_path_equiv.inducts, auto)
-
-lemma algorithmic_monotonicity:
-  fixes \<Gamma>':: "(name\<times>ty) list"
-  shows "\<Gamma> \<turnstile> s <=> t : T \<Longrightarrow> \<Gamma>\<lless>\<Gamma>' \<Longrightarrow> \<Gamma>' \<turnstile> s <=> t : T"
-  and "\<Gamma> \<turnstile> s \<leftrightarrow> t : T \<Longrightarrow> \<Gamma>\<lless>\<Gamma>' \<Longrightarrow> \<Gamma>' \<turnstile> s \<leftrightarrow> t : T"
-proof (nominal_induct \<Gamma> s t T and \<Gamma> s t T avoiding: \<Gamma>' rule: alg_equiv_alg_path_equiv_strong_inducts)
-  case (QAT_Arrow x \<Gamma> s t T1 T2 \<Gamma>')
-  have fs:"x\<sharp>\<Gamma>" "x\<sharp>s" "x\<sharp>t" by fact
-  have h2:"\<Gamma>\<lless>\<Gamma>'" by fact
-  have ih:"\<And>\<Gamma>'. \<lbrakk>(x,T1)#\<Gamma> \<lless> \<Gamma>'\<rbrakk>  \<Longrightarrow> \<Gamma>' \<turnstile> App s (Var x) <=> App t (Var x) : T2" by fact
-  have "x\<sharp>\<Gamma>'" by fact
-  then have sub:"(x,T1)#\<Gamma> \<lless> (x,T1)#\<Gamma>'" using h2 by auto
-  then have "(x,T1)#\<Gamma>' \<turnstile> App s (Var x) <=> App t (Var x) : T2" using ih by auto
-  then show "\<Gamma>' \<turnstile> s <=> t : T1\<rightarrow>T2" using sub fs by auto
-qed (auto)
-
-text {* Logical equivalence. *}
-
-function log_equiv :: "((name\<times>ty) list \<Rightarrow> trm \<Rightarrow> trm \<Rightarrow> ty \<Rightarrow> bool)"   
-                      ("_ \<turnstile> _ is _ : _" [60,60,60,60] 60) 
-where    
-   "\<Gamma> \<turnstile> s is t : TUnit = valid \<Gamma>"
- | "\<Gamma> \<turnstile> s is t : TBase = \<Gamma> \<turnstile> s <=> t : TBase"
- | "\<Gamma> \<turnstile> s is t : (T1 \<rightarrow> T2) =  
-           (valid \<Gamma> \<and> (\<forall>\<Gamma>' s' t'. \<Gamma>\<lless>\<Gamma>' \<longrightarrow> \<Gamma>' \<turnstile> s' is t' : T1 \<longrightarrow>  (\<Gamma>' \<turnstile> (App s s') is (App t t') : T2)))"
-apply (auto simp add: ty.inject)
-apply (subgoal_tac "(\<exists>T1 T2. b=T1 \<rightarrow> T2) \<or> b=TUnit \<or> b=TBase" )
-apply (force)
-apply (rule ty_cases)
-done
-
-termination
-apply(relation "measure (\<lambda>(_,_,_,T). size T)")
-apply(auto)
-done
-
-lemma log_equiv_valid: 
-  assumes "\<Gamma> \<turnstile> s is t : T"
-  shows "valid \<Gamma>"
-using assms 
-by (induct rule: log_equiv.induct,auto elim: alg_equiv_valid)
-
-lemma logical_monotonicity :
- fixes T::ty
- assumes "\<Gamma> \<turnstile> s is t : T" "\<Gamma>\<lless>\<Gamma>'" 
- shows "\<Gamma>' \<turnstile> s is t : T"
-using assms
-proof (induct arbitrary: \<Gamma>' rule: log_equiv.induct)
-  case (2 \<Gamma> s t \<Gamma>')
-  then show "\<Gamma>' \<turnstile> s is t : TBase" using algorithmic_monotonicity by auto
-next
-  case (3 \<Gamma> s t T1 T2 \<Gamma>')
-  have h1:"\<Gamma> \<turnstile> s is t : T1\<rightarrow>T2" by fact
-  have h2:"\<Gamma>\<lless>\<Gamma>'" by fact
-  {
-    fix \<Gamma>'' s' t'
-    assume "\<Gamma>'\<lless>\<Gamma>''" "\<Gamma>'' \<turnstile> s' is t' : T1"
-    then have "\<Gamma>'' \<turnstile> (App s s') is (App t t') : T2" using h1 h2 by auto
-  }
-  then show "\<Gamma>' \<turnstile> s is t : T1\<rightarrow>T2" using h2 by auto
-qed (auto)
-  
 lemma forget: 
   fixes x::"name"
   and   L::"trm"
@@ -766,17 +485,17 @@ by (nominal_induct L avoiding: x P rule: trm.induct)
 
 lemma subst_fun_eq:
   fixes u::trm
-  assumes h:"[x].t1 = [y].t2"
-  shows "t1[x::=u] = t2[y::=u]"
+  assumes h:"[x].t\<^isub>1 = [y].t\<^isub>2"
+  shows "t\<^isub>1[x::=u] = t\<^isub>2[y::=u]"
 proof -
   { 
-    assume "x=y" and "t1=t2"
+    assume "x=y" and "t\<^isub>1=t\<^isub>2"
     then have ?thesis using h by simp
   }
   moreover 
   {
-    assume h1:"x \<noteq> y" and h2:"t1=[(x,y)] \<bullet> t2" and h3:"x \<sharp> t2"
-    then have "([(x,y)] \<bullet> t2)[x::=u] = t2[y::=u]" by (simp add: subst_rename)
+    assume h1:"x \<noteq> y" and h2:"t\<^isub>1=[(x,y)] \<bullet> t\<^isub>2" and h3:"x \<sharp> t\<^isub>2"
+    then have "([(x,y)] \<bullet> t\<^isub>2)[x::=u] = t\<^isub>2[y::=u]" by (simp add: subst_rename)
     then have ?thesis using h2 by simp 
   }
   ultimately show ?thesis using alpha h by blast
@@ -787,7 +506,7 @@ lemma psubst_empty[simp]:
   by (nominal_induct t rule: trm.induct) (auto simp add: fresh_list_nil)
 
 lemma psubst_subst_psubst:
-  assumes h:"c \<sharp> \<theta>"
+  assumes h:"c\<sharp>\<theta>"
   shows "\<theta><t>[c::=s] = (c,s)#\<theta><t>"
   using h
 by (nominal_induct t avoiding: \<theta> c s rule: trm.induct)
@@ -830,13 +549,473 @@ next
   ultimately have "\<theta><(Lam [n].t)[x::=u]> = (Lam [n].\<theta><t>)[x::=\<theta><u>]" using fs by auto
   then show "\<theta><(Lam [n].t)[x::=u]> = \<theta><Lam [n].t>[x::=\<theta><u>]" using fs by auto
 qed (auto)
+
+text {* 
+\section{Equivalence}
+\subsection{Definition of the equivalence relation}
+ *}
+
+(*<*)
+inductive2
+  equiv_def :: "(name\<times>ty) list\<Rightarrow>trm\<Rightarrow>trm\<Rightarrow>ty\<Rightarrow>bool" ("_ \<turnstile> _ \<equiv> _ : _" [60,60] 60) 
+where
+  Q_Refl[intro]:  "\<Gamma> \<turnstile> t : T \<Longrightarrow> \<Gamma> \<turnstile> t \<equiv> t : T"
+| Q_Symm[intro]:  "\<Gamma> \<turnstile> t \<equiv> s : T \<Longrightarrow> \<Gamma> \<turnstile> s \<equiv> t : T"
+| Q_Trans[intro]: "\<lbrakk>\<Gamma> \<turnstile> s \<equiv> t : T; \<Gamma> \<turnstile> t \<equiv> u : T\<rbrakk> \<Longrightarrow>  \<Gamma> \<turnstile> s \<equiv> u : T"
+| Q_Abs[intro]:   "\<lbrakk>x\<sharp>\<Gamma>; (x,T\<^isub>1)#\<Gamma> \<turnstile> s\<^isub>2 \<equiv> t\<^isub>2 : T\<^isub>2\<rbrakk> \<Longrightarrow> \<Gamma> \<turnstile> Lam [x]. s\<^isub>2 \<equiv>  Lam [x]. t\<^isub>2 : T\<^isub>1 \<rightarrow> T\<^isub>2"
+| Q_App[intro]:   "\<lbrakk>\<Gamma> \<turnstile> s\<^isub>1 \<equiv> t\<^isub>1 : T\<^isub>1 \<rightarrow> T\<^isub>2 ; \<Gamma> \<turnstile> s\<^isub>2 \<equiv> t\<^isub>2 : T\<^isub>1\<rbrakk> \<Longrightarrow>  \<Gamma> \<turnstile> App s\<^isub>1 s\<^isub>2 \<equiv> App t\<^isub>1 t\<^isub>2 : T\<^isub>2"
+| Q_Beta[intro]:  "\<lbrakk>x\<sharp>(\<Gamma>,s\<^isub>2,t\<^isub>2); (x,T\<^isub>1)#\<Gamma> \<turnstile> s12 \<equiv> t12 : T\<^isub>2 ; \<Gamma> \<turnstile> s\<^isub>2 \<equiv> t\<^isub>2 : T\<^isub>1\<rbrakk> 
+                   \<Longrightarrow>  \<Gamma> \<turnstile> App (Lam [x]. s12) s\<^isub>2 \<equiv>  t12[x::=t\<^isub>2] : T\<^isub>2"
+| Q_Ext[intro]:   "\<lbrakk>x\<sharp>(\<Gamma>,s,t); (x,T\<^isub>1)#\<Gamma> \<turnstile> App s (Var x) \<equiv> App t (Var x) : T\<^isub>2\<rbrakk> 
+                   \<Longrightarrow> \<Gamma> \<turnstile> s \<equiv> t : T\<^isub>1 \<rightarrow> T\<^isub>2"
+(*>*)
+
+text {* 
+\begin{center}
+\isastyle
+@{thm[mode=Rule] Q_Refl[no_vars]}{\sc{Q\_Refl}}\qquad
+@{thm[mode=Rule] Q_Symm[no_vars]}{\sc{Q\_Symm}}\\
+@{thm[mode=Rule] Q_Trans[no_vars]}{\sc{Q\_Trans}}\\
+@{thm[mode=Rule] Q_App[no_vars]}{\sc{Q\_App}}\\
+@{thm[mode=Rule] Q_Abs[no_vars]}{\sc{Q\_Abs}}\\
+@{thm[mode=Rule] Q_Beta[no_vars]}{\sc{Q\_Beta}}\\
+@{thm[mode=Rule] Q_Ext[no_vars]}{\sc{Q\_Ext}}\\
+\end{center}
+*}
+
+text {* It is now a tradition, we derive the lemma about validity, and we generate the equivariance lemma. *}
+
+lemma equiv_def_valid:
+  assumes "\<Gamma> \<turnstile> t \<equiv> s : T"
+  shows "valid \<Gamma>"
+using assms by (induct,auto elim:typing_valid)
+
+nominal_inductive equiv_def
+
+text{*
+\subsection{Strong induction principle for the equivalence relation}
+*}
+
+lemma equiv_def_strong_induct
+  [consumes 1, case_names Q_Refl Q_Symm Q_Trans Q_Abs Q_App Q_Beta Q_Ext]:
+  fixes c::"'a::fs_name"
+  assumes a0: "\<Gamma> \<turnstile> s \<equiv> t : T" 
+  and     a1: "\<And>\<Gamma> t T c.  \<Gamma> \<turnstile> t : T  \<Longrightarrow> P c \<Gamma> t t T"
+  and     a2: "\<And>\<Gamma> t s T c. \<lbrakk>\<And>d. P d \<Gamma> t s T\<rbrakk> \<Longrightarrow>  P c \<Gamma> s t T"
+  and     a3: "\<And>\<Gamma> s t T u c. \<lbrakk>\<And>d. P d \<Gamma> s t T; \<And>d. P d \<Gamma> t u T\<rbrakk> 
+               \<Longrightarrow> P c \<Gamma> s u T"
+  and     a4: "\<And>x \<Gamma> T\<^isub>1 s\<^isub>2 t\<^isub>2 T\<^isub>2 c. \<lbrakk>x\<sharp>\<Gamma>; x\<sharp>c; \<And>d. P d ((x,T\<^isub>1)#\<Gamma>) s\<^isub>2 t\<^isub>2 T\<^isub>2\<rbrakk>
+               \<Longrightarrow> P c \<Gamma> (Lam [x].s\<^isub>2) (Lam [x].t\<^isub>2) (T\<^isub>1\<rightarrow>T\<^isub>2)"
+  and     a5: "\<And>\<Gamma> s\<^isub>1 t\<^isub>1 T\<^isub>1 T\<^isub>2 s\<^isub>2 t\<^isub>2 c. \<lbrakk>\<And>d. P d \<Gamma> s\<^isub>1 t\<^isub>1 (T\<^isub>1\<rightarrow>T\<^isub>2); \<And>d. P d \<Gamma> s\<^isub>2 t\<^isub>2 T\<^isub>1\<rbrakk> 
+               \<Longrightarrow> P c \<Gamma> (App s\<^isub>1 s\<^isub>2) (App t\<^isub>1 t\<^isub>2) T\<^isub>2"
+  and     a6: "\<And>x \<Gamma> T\<^isub>1 s12 t12 T\<^isub>2 s\<^isub>2 t\<^isub>2 c.
+               \<lbrakk>x\<sharp>(\<Gamma>,s\<^isub>2,t\<^isub>2); x\<sharp>c; \<And>d. P d ((x,T\<^isub>1)#\<Gamma>) s12 t12 T\<^isub>2; \<And>d. P d \<Gamma> s\<^isub>2 t\<^isub>2 T\<^isub>1\<rbrakk> 
+               \<Longrightarrow> P c \<Gamma> (App (Lam [x].s12) s\<^isub>2) (t12[x::=t\<^isub>2]) T\<^isub>2"
+  and     a7: "\<And>x \<Gamma> s t T\<^isub>1 T\<^isub>2 c.
+               \<lbrakk>x\<sharp>(\<Gamma>,s,t); \<And>d. P d ((x,T\<^isub>1)#\<Gamma>) (App s (Var x)) (App t (Var x)) T\<^isub>2\<rbrakk>
+               \<Longrightarrow> P c \<Gamma> s t (T\<^isub>1\<rightarrow>T\<^isub>2)"
+ shows "P c \<Gamma>  s t T"
+proof -
+  from a0 have "\<And>(pi::name prm) c. P c (pi\<bullet>\<Gamma>) (pi\<bullet>s) (pi\<bullet>t) (pi\<bullet>T)" 
+    proof(induct)
+      case (Q_Refl \<Gamma> t T pi c)
+      then show "P c (pi\<bullet>\<Gamma>) (pi\<bullet>t) (pi\<bullet>t) (pi\<bullet>T)" using a1 by (simp only: eqvt)
+    next
+      case (Q_Symm \<Gamma> t s T pi c)
+      then show "P c (pi\<bullet>\<Gamma>) (pi\<bullet>s) (pi\<bullet>t) (pi\<bullet>T)" using a2 by (simp only: equiv_def_eqvt)
+    next
+      case (Q_Trans \<Gamma> s t T u pi c)
+      then show " P c (pi\<bullet>\<Gamma>) (pi\<bullet>s) (pi\<bullet>u) (pi\<bullet>T)" using a3 by (blast intro: equiv_def_eqvt)
+    next
+      case (Q_App \<Gamma> s\<^isub>1 t\<^isub>1 T\<^isub>1 T\<^isub>2 s\<^isub>2 t\<^isub>2 pi c)
+      then show "P c (pi\<bullet>\<Gamma>) (pi\<bullet>App s\<^isub>1 s\<^isub>2) (pi\<bullet>App t\<^isub>1 t\<^isub>2) (pi\<bullet>T\<^isub>2)" using a5 
+	by (simp only: eqvt) (blast)
+    next
+      case (Q_Ext x \<Gamma> s t T\<^isub>1 T\<^isub>2 pi c)
+      then show "P c (pi\<bullet>\<Gamma>) (pi\<bullet>s) (pi\<bullet>t) (pi\<bullet>T\<^isub>1\<rightarrow>T\<^isub>2)"  
+	by (auto intro!: a7 simp add: fresh_bij)
+    next
+      case (Q_Abs x \<Gamma> T\<^isub>1 s\<^isub>2 t\<^isub>2 T\<^isub>2 pi c)
+      obtain y::"name" where fs: "y\<sharp>(pi\<bullet>x,pi\<bullet>s\<^isub>2,pi\<bullet>t\<^isub>2,pi\<bullet>\<Gamma>,c)" by (rule exists_fresh[OF fs_name1])
+      let ?sw="[(pi\<bullet>x,y)]"
+      let ?pi'="?sw@pi"
+      have f1: "x\<sharp>\<Gamma>" by fact
+      have f2: "(pi\<bullet>x)\<sharp>(pi\<bullet>\<Gamma>)" using f1 by (simp add: fresh_bij)
+      have f3: "y\<sharp>?pi'\<bullet>\<Gamma>" using f1 by (auto simp add: pt_name2 fresh_left calc_atm perm_pi_simp)
+      have ih1: "\<And>c. P c (?pi'\<bullet>((x,T\<^isub>1)#\<Gamma>)) (?pi'\<bullet>s\<^isub>2) (?pi'\<bullet>t\<^isub>2) (?pi'\<bullet>T\<^isub>2)" by fact
+      then have "\<And>c. P c ((y,T\<^isub>1)#(?pi'\<bullet>\<Gamma>)) (?pi'\<bullet>s\<^isub>2) (?pi'\<bullet>t\<^isub>2) T\<^isub>2" by (simp add: calc_atm)
+      then have "P c  (?pi'\<bullet>\<Gamma>) (?pi'\<bullet>Lam [x].s\<^isub>2) (?pi'\<bullet>Lam [x].t\<^isub>2) (T\<^isub>1\<rightarrow>T\<^isub>2)" using a4 f3 fs
+	by (simp add: calc_atm)
+      then have "P c (?sw\<bullet>pi\<bullet>\<Gamma>) (?sw\<bullet>Lam [(pi\<bullet>x)].(pi\<bullet>s\<^isub>2)) (?sw\<bullet>Lam [(pi\<bullet>x)].(pi\<bullet>t\<^isub>2)) (T\<^isub>1\<rightarrow>T\<^isub>2)" 
+	by (simp del: append_Cons add: calc_atm pt_name2)
+      moreover have "(?sw\<bullet>(pi\<bullet>\<Gamma>)) = (pi\<bullet>\<Gamma>)" 
+	by (rule perm_fresh_fresh) (simp_all add: fs f2)
+      moreover have "(?sw\<bullet>(Lam [(pi\<bullet>x)].(pi\<bullet>s\<^isub>2))) = Lam [(pi\<bullet>x)].(pi\<bullet>s\<^isub>2)" 
+	by (rule perm_fresh_fresh) (simp_all add: fs f2 abs_fresh)
+      moreover have "(?sw\<bullet>(Lam [(pi\<bullet>x)].(pi\<bullet>t\<^isub>2))) = Lam [(pi\<bullet>x)].(pi\<bullet>t\<^isub>2)" 
+	by (rule perm_fresh_fresh) (simp_all add: fs f2 abs_fresh)
+      ultimately have "P c (pi\<bullet>\<Gamma>) (Lam [(pi\<bullet>x)].(pi\<bullet>s\<^isub>2)) (Lam [(pi\<bullet>x)].(pi\<bullet>t\<^isub>2)) (T\<^isub>1\<rightarrow>T\<^isub>2)" by simp
+      then show  "P c (pi\<bullet>\<Gamma>) (pi\<bullet>Lam [x].s\<^isub>2) (pi\<bullet>Lam [x].t\<^isub>2) (pi\<bullet>T\<^isub>1\<rightarrow>T\<^isub>2)" by simp 
+    next 
+      case (Q_Beta x \<Gamma> s\<^isub>2 t\<^isub>2 T\<^isub>1 s12 t12 T\<^isub>2 pi c) 
+      obtain y::"name" where fs: "y\<sharp>(pi\<bullet>x,pi\<bullet>s12,pi\<bullet>t12,pi\<bullet>s\<^isub>2,pi\<bullet>t\<^isub>2,pi\<bullet>\<Gamma>,c)" 
+	by (rule exists_fresh[OF fs_name1])
+      let ?sw="[(pi\<bullet>x,y)]"
+      let ?pi'="?sw@pi"
+      have f1: "x\<sharp>(\<Gamma>,s\<^isub>2,t\<^isub>2)" by fact 
+      have f2: "(pi\<bullet>x)\<sharp>(pi\<bullet>(\<Gamma>,s\<^isub>2,t\<^isub>2))" using f1 by (simp add: fresh_bij)
+      have f3: "y\<sharp>(?pi'\<bullet>(\<Gamma>,s\<^isub>2,t\<^isub>2))" using f1 
+	by (auto simp add: pt_name2 fresh_left calc_atm perm_pi_simp fresh_prod)
+      have ih1: "\<And>c. P c (?pi'\<bullet>((x,T\<^isub>1)#\<Gamma>)) (?pi'\<bullet>s12) (?pi'\<bullet>t12) (?pi'\<bullet>T\<^isub>2)" by fact
+      then have "\<And>c. P c ((y,T\<^isub>1)#(?pi'\<bullet>\<Gamma>)) (?pi'\<bullet>s12) (?pi'\<bullet>t12) (?pi'\<bullet>T\<^isub>2)" by (simp add: calc_atm)
+      moreover
+      have ih2: "\<And>c. P c (?pi'\<bullet>\<Gamma>) (?pi'\<bullet>s\<^isub>2) (?pi'\<bullet>t\<^isub>2) (?pi'\<bullet>T\<^isub>1)" by fact
+      ultimately have "P c  (?pi'\<bullet>\<Gamma>) (?pi'\<bullet>(App (Lam [x].s12) s\<^isub>2)) (?pi'\<bullet>(t12[x::=t\<^isub>2])) (?pi'\<bullet>T\<^isub>2)" 
+	using a6 f3 fs by (force simp add: subst_eqvt calc_atm del: perm_ty)
+      then have "P c (?sw\<bullet>pi\<bullet>\<Gamma>) (?sw\<bullet>(App (Lam [(pi\<bullet>x)].(pi\<bullet>s12)) (pi\<bullet>s\<^isub>2))) 
+	(?sw\<bullet>((pi\<bullet>t12)[(pi\<bullet>x)::=(pi\<bullet>t\<^isub>2)])) T\<^isub>2" 
+	by (simp del: append_Cons add: calc_atm pt_name2 subst_eqvt)
+      moreover have "(?sw\<bullet>(pi\<bullet>\<Gamma>)) = (pi\<bullet>\<Gamma>)" 
+	by (rule perm_fresh_fresh) (simp_all add: fs[simplified] f2[simplified])
+      moreover have "(?sw\<bullet>(App (Lam [(pi\<bullet>x)].(pi\<bullet>s12)) (pi\<bullet>s\<^isub>2))) = App (Lam [(pi\<bullet>x)].(pi\<bullet>s12)) (pi\<bullet>s\<^isub>2)" 
+	by (rule perm_fresh_fresh) (simp_all add: fs[simplified] f2[simplified] abs_fresh)
+      moreover have "(?sw\<bullet>((pi\<bullet>t12)[(pi\<bullet>x)::=(pi\<bullet>t\<^isub>2)])) = ((pi\<bullet>t12)[(pi\<bullet>x)::=(pi\<bullet>t\<^isub>2)])" 
+	by (rule perm_fresh_fresh) 
+	   (simp_all add: fs[simplified] f2[simplified] fresh_subst fresh_subst'')
+      ultimately have "P c (pi\<bullet>\<Gamma>) (App (Lam [(pi\<bullet>x)].(pi\<bullet>s12)) (pi\<bullet>s\<^isub>2)) ((pi\<bullet>t12)[(pi\<bullet>x)::=(pi\<bullet>t\<^isub>2)]) T\<^isub>2"
+	by simp
+      then show "P c (pi\<bullet>\<Gamma>) (pi\<bullet>App (Lam [x].s12) s\<^isub>2) (pi\<bullet>t12[x::=t\<^isub>2]) (pi\<bullet>T\<^isub>2)" by (simp add: subst_eqvt)
+    qed
+  then have "P c (([]::name prm)\<bullet>\<Gamma>) (([]::name prm)\<bullet>s) (([]::name prm)\<bullet>t) (([]::name prm)\<bullet>T)" by blast
+  then show "P c \<Gamma> s t T" by simp
+qed
+
+
+text {* \section{Type-driven equivalence algorithm} 
+
+We follow the original presentation. The algorithm is described using inference rules only.
+
+*}
+
+text {* \subsection{Weak head reduction} *}
+
+(*<*)
+inductive2
+  whr_def :: "trm\<Rightarrow>trm\<Rightarrow>bool" ("_ \<leadsto> _" [80,80] 80) 
+where
+  QAR_Beta[intro]: "App (Lam [x]. t12) t\<^isub>2 \<leadsto> t12[x::=t\<^isub>2]"
+| QAR_App[intro]: "t1 \<leadsto> t1' \<Longrightarrow> App t1 t\<^isub>2 \<leadsto> App t1' t\<^isub>2"
+(*>*)
+
+text {* 
+\begin{figure}
+\begin{center}
+\isastyle
+@{thm[mode=Rule] QAR_Beta[no_vars]}{\sc{QAR\_Beta}} \qquad
+@{thm[mode=Rule] QAR_App[no_vars]}{\sc{QAR\_App}}
+\end{center}
+\end{figure}
+*}
+
+text {* \subsubsection{Inversion lemma for weak head reduction} *}
+
+declare trm.inject  [simp add]
+declare ty.inject  [simp add]
+
+inductive_cases2 whr_Gen[elim]: "t \<leadsto> t'"
+inductive_cases2 whr_Lam[elim]: "Lam [x].t \<leadsto> t'"
+inductive_cases2 whr_App_Lam[elim]: "App (Lam [x].t12) t2 \<leadsto> t"
+inductive_cases2 whr_Var[elim]: "Var x \<leadsto> t"
+inductive_cases2 whr_Const[elim]: "Const n \<leadsto> t"
+inductive_cases2 whr_App[elim]: "App p q \<leadsto> t"
+inductive_cases2 whr_Const_Right[elim]: "t \<leadsto> Const n"
+inductive_cases2 whr_Var_Right[elim]: "t \<leadsto> Var x"
+inductive_cases2 whr_App_Right[elim]: "t \<leadsto> App p q"
+
+declare trm.inject  [simp del]
+declare ty.inject  [simp del]
+
+nominal_inductive whr_def
+
+text {* 
+\subsection{Weak head normalization} 
+\subsubsection{Definition of the normal form}
+*}
+
+abbreviation 
+ nf :: "trm \<Rightarrow> bool" ("_ \<leadsto>|" [100] 100)
+where
+  "t\<leadsto>|  \<equiv> \<not>(\<exists> u. t \<leadsto> u)" 
+
+text{* \subsubsection{Definition of weak head normal form} *}
+
+(*<*)
+inductive2
+  whn_def :: "trm\<Rightarrow>trm\<Rightarrow>bool" ("_ \<Down> _" [80,80] 80) 
+where
+  QAN_Reduce[intro]: "\<lbrakk>s \<leadsto> t; t \<Down> u\<rbrakk> \<Longrightarrow> s \<Down> u"
+| QAN_Normal[intro]: "t\<leadsto>|  \<Longrightarrow> t \<Down> t"
+
+(*>*)
+
+text {* 
+\begin{center}
+@{thm[mode=Rule] QAN_Reduce[no_vars]}{\sc{QAN\_Reduce}}\qquad
+@{thm[mode=Rule] QAN_Normal[no_vars]}{\sc{QAN\_Normal}}
+\end{center}
+*}
+
+lemma whn_eqvt[eqvt]:
+  fixes pi::"name prm"
+  assumes a: "t \<Down> t'"
+  shows "(pi\<bullet>t) \<Down> (pi\<bullet>t')"
+using a
+apply(induct)
+apply(rule QAN_Reduce)
+apply(rule whr_def_eqvt)
+apply(assumption)+
+apply(rule QAN_Normal)
+apply(auto)
+apply(drule_tac pi="rev pi" in whr_def_eqvt)
+apply(perm_simp)
+done
+
+text {* \subsection{Algorithmic term equivalence and algorithmic path equivalence} *}
+
+(*<*)
+inductive2
+  alg_equiv :: "(name\<times>ty) list\<Rightarrow>trm\<Rightarrow>trm\<Rightarrow>ty\<Rightarrow>bool" ("_ \<turnstile> _ \<Leftrightarrow> _ : _" [60,60] 60) 
+and
+  alg_path_equiv :: "(name\<times>ty) list\<Rightarrow>trm\<Rightarrow>trm\<Rightarrow>ty\<Rightarrow>bool" ("_ \<turnstile> _ \<leftrightarrow> _ : _" [60,60] 60) 
+where
+  QAT_Base[intro]:  "\<lbrakk>s \<Down> p; t \<Down> q; \<Gamma> \<turnstile> p \<leftrightarrow> q : TBase \<rbrakk> \<Longrightarrow> \<Gamma> \<turnstile> s \<Leftrightarrow> t : TBase"
+| QAT_Arrow[intro]: "\<lbrakk>x\<sharp>\<Gamma>; x\<sharp>s; x\<sharp>t; (x,T\<^isub>1)#\<Gamma> \<turnstile> App s (Var x) \<Leftrightarrow> App t (Var x) : T\<^isub>2\<rbrakk> 
+                     \<Longrightarrow> \<Gamma> \<turnstile> s \<Leftrightarrow> t : T\<^isub>1 \<rightarrow> T\<^isub>2"
+| QAT_One[intro]:   "valid \<Gamma> \<Longrightarrow> \<Gamma> \<turnstile> s \<Leftrightarrow> t : TUnit"
+| QAP_Var[intro]:   "\<lbrakk>valid \<Gamma>;(x,T) \<in> set \<Gamma>\<rbrakk> \<Longrightarrow> \<Gamma> \<turnstile> Var x \<leftrightarrow> Var x : T"
+| QAP_App[intro]:   "\<lbrakk>\<Gamma> \<turnstile> p \<leftrightarrow> q : T\<^isub>1 \<rightarrow> T\<^isub>2; \<Gamma> \<turnstile> s \<Leftrightarrow> t : T\<^isub>1 \<rbrakk> \<Longrightarrow> \<Gamma> \<turnstile> App p s \<leftrightarrow> App q t : T\<^isub>2"
+| QAP_Const[intro]: "valid \<Gamma> \<Longrightarrow> \<Gamma> \<turnstile> Const n \<leftrightarrow> Const n : TBase"
+(*>*)
+
+text {* 
+\begin{center}
+@{thm[mode=Rule] QAT_Base[no_vars]}{\sc{QAT\_Base}}\\
+@{thm[mode=Rule] QAT_Arrow[no_vars]}{\sc{QAT\_Arrow}}\\
+@{thm[mode=Rule] QAP_Var[no_vars]}{\sc{QAP\_Var}}\\
+@{thm[mode=Rule] QAP_App[no_vars]}{\sc{QAP\_App}}\\
+@{thm[mode=Rule] QAP_Const[no_vars]}{\sc{QAP\_Const}}\\
+\end{center}
+*}
+
+text {* Again we generate the equivariance lemma. *}
+
+nominal_inductive  alg_equiv
+
+text {* \subsubsection{Strong induction principle for algorithmic term and path equivalences} *}
+
+lemma alg_equiv_alg_path_equiv_strong_induct
+  [case_names QAT_Base QAT_Arrow QAT_One QAP_Var QAP_App QAP_Const]:
+  fixes c::"'a::fs_name"
+  assumes a1: "\<And>s p t q \<Gamma> c. \<lbrakk>s \<Down> p; t \<Down> q; \<Gamma> \<turnstile> p \<leftrightarrow> q : TBase; \<And>d. P2 d \<Gamma> p q TBase\<rbrakk> 
+               \<Longrightarrow> P1 c \<Gamma> s t TBase"
+  and     a2: "\<And>x \<Gamma> s t T\<^isub>1 T\<^isub>2 c.
+               \<lbrakk>x\<sharp>\<Gamma>; x\<sharp>s; x\<sharp>t; x\<sharp>c; (x,T\<^isub>1)#\<Gamma> \<turnstile> App s (Var x) \<Leftrightarrow> App t (Var x) : T\<^isub>2;
+               \<And>d. P1 d ((x,T\<^isub>1)#\<Gamma>) (App s (Var x)) (App t (Var x)) T\<^isub>2\<rbrakk>
+               \<Longrightarrow> P1 c \<Gamma> s t (T\<^isub>1\<rightarrow>T\<^isub>2)"
+  and     a3: "\<And>\<Gamma> s t c. valid \<Gamma> \<Longrightarrow> P1 c \<Gamma> s t TUnit"
+  and     a4: "\<And>\<Gamma> x T c. \<lbrakk>valid \<Gamma>; (x,T) \<in> set \<Gamma>\<rbrakk> \<Longrightarrow> P2 c \<Gamma> (Var x) (Var x) T"
+  and     a5: "\<And>\<Gamma> p q T\<^isub>1 T\<^isub>2 s t c.
+               \<lbrakk>\<Gamma> \<turnstile> p \<leftrightarrow> q : T\<^isub>1\<rightarrow>T\<^isub>2; \<And>d. P2 d \<Gamma> p q (T\<^isub>1\<rightarrow>T\<^isub>2); \<Gamma> \<turnstile> s \<Leftrightarrow> t : T\<^isub>1; \<And>d. P1 d \<Gamma> s t T\<^isub>1\<rbrakk>
+               \<Longrightarrow> P2 c \<Gamma> (App p s) (App q t) T\<^isub>2"
+  and     a6: "\<And>\<Gamma> n c. valid \<Gamma> \<Longrightarrow> P2 c \<Gamma> (Const n) (Const n) TBase"
+  shows "(\<Gamma> \<turnstile> s \<Leftrightarrow> t : T \<longrightarrow>P1 c \<Gamma> s t T) \<and> (\<Gamma>' \<turnstile> s' \<leftrightarrow> t' : T' \<longrightarrow> P2 c \<Gamma>' s' t' T')"
+proof -
+  have "(\<Gamma> \<turnstile> s \<Leftrightarrow> t : T \<longrightarrow> (\<forall>c (pi::name prm). P1 c (pi\<bullet>\<Gamma>) (pi\<bullet>s) (pi\<bullet>t) T)) \<and> 
+        (\<Gamma>' \<turnstile> s' \<leftrightarrow> t' : T' \<longrightarrow> (\<forall>c (pi::name prm). P2 c (pi\<bullet>\<Gamma>') (pi\<bullet>s') (pi\<bullet>t') T'))"
+  proof(induct rule: alg_equiv_alg_path_equiv.induct)
+    case (QAT_Base s q t p \<Gamma>)
+    then show "\<forall>c (pi::name prm). P1 c (pi\<bullet>\<Gamma>) (pi\<bullet>s) (pi\<bullet>t) TBase"
+      apply(auto)
+      apply(rule_tac p="pi\<bullet>q" and q="pi\<bullet>p" in  a1)
+      apply(simp_all add: eqvt[simplified])
+      done
+  next
+    case (QAT_Arrow x \<Gamma> s t T\<^isub>1 T\<^isub>2)
+    show ?case
+    proof (rule allI, rule allI)
+      fix c::"'a::fs_name" and pi::"name prm"
+      obtain y::"name" where fs: "y\<sharp>(pi\<bullet>s,pi\<bullet>t,pi\<bullet>\<Gamma>,c)" by (rule exists_fresh[OF fs_name1])
+      let ?sw="[(pi\<bullet>x,y)]"
+      let ?pi'="?sw@pi"
+      have f0: "x\<sharp>\<Gamma>" "x\<sharp>s" "x\<sharp>t" by fact
+      then have f1: "x\<sharp>(\<Gamma>,s,t)" by simp
+      have f2: "(pi\<bullet>x)\<sharp>(pi\<bullet>(\<Gamma>,s,t))" using f1 by (simp add: fresh_bij)
+      have f3: "y\<sharp>?pi'\<bullet>(\<Gamma>,s,t)" using f1 
+	by (simp only: pt_name2 fresh_left, auto simp add: perm_pi_simp calc_atm)
+      then have f3': "y\<sharp>?pi'\<bullet>\<Gamma>" "y\<sharp>?pi'\<bullet>s" "y\<sharp>?pi'\<bullet>t" by (auto simp add: fresh_prod)
+      have pr1: "(x,T\<^isub>1)#\<Gamma> \<turnstile> App s (Var x) \<Leftrightarrow> App t (Var x) : T\<^isub>2" by fact
+      then have "?pi'\<bullet> ((x,T\<^isub>1)#\<Gamma> \<turnstile> App s (Var x) \<Leftrightarrow> App t (Var x) : T\<^isub>2)" using perm_bool by simp
+      then have "(?pi'\<bullet>((x,T\<^isub>1)#\<Gamma>)) \<turnstile> (?pi'\<bullet>(App s (Var x))) \<Leftrightarrow> (?pi'\<bullet>(App t (Var x))) : (?pi'\<bullet>T\<^isub>2)" 
+	by (auto simp add: eqvt)
+      then have "(y,T\<^isub>1)#(?pi'\<bullet>\<Gamma>) \<turnstile> (App (?pi'\<bullet>s) (Var y)) \<Leftrightarrow> (App (?pi'\<bullet>t) (Var y)) : T\<^isub>2" 
+	by (simp add: calc_atm)
+      moreover    
+      have ih1: "\<forall>c (pi::name prm).  P1 c (pi\<bullet>((x,T\<^isub>1)#\<Gamma>)) (pi\<bullet>App s (Var x)) (pi\<bullet>App t (Var x)) T\<^isub>2"
+	by fact
+      then have "\<And>c.  P1 c (?pi'\<bullet>((x,T\<^isub>1)#\<Gamma>)) (?pi'\<bullet>App s (Var x)) (?pi'\<bullet>App t (Var x)) T\<^isub>2"
+	by auto
+      then have "\<And>c.  P1 c ((y,T\<^isub>1)#(?pi'\<bullet>\<Gamma>)) (App (?pi'\<bullet>s) (Var y)) (App (?pi'\<bullet>t) (Var y)) T\<^isub>2"
+	by (simp add: calc_atm)     
+      ultimately have "P1 c (?pi'\<bullet>\<Gamma>) (?pi'\<bullet>s) (?pi'\<bullet>t) (T\<^isub>1\<rightarrow>T\<^isub>2)" using a2 f3' fs by simp
+      then have "P1 c (?sw\<bullet>pi\<bullet>\<Gamma>) (?sw\<bullet>pi\<bullet>s) (?sw\<bullet>pi\<bullet>t) (T\<^isub>1\<rightarrow>T\<^isub>2)" 
+	by (simp del: append_Cons add: calc_atm pt_name2)
+      moreover have "(?sw\<bullet>(pi\<bullet>\<Gamma>)) = (pi\<bullet>\<Gamma>)" 
+	by (rule perm_fresh_fresh) (simp_all add: fs[simplified] f2[simplified])
+      moreover have "(?sw\<bullet>(pi\<bullet>s)) = (pi\<bullet>s)" 
+	by (rule perm_fresh_fresh) (simp_all add: fs[simplified] f2[simplified])
+      moreover have "(?sw\<bullet>(pi\<bullet>t)) = (pi\<bullet>t)" 
+	by (rule perm_fresh_fresh) (simp_all add: fs[simplified] f2[simplified])
+      ultimately show "P1 c (pi\<bullet>\<Gamma>) (pi\<bullet>s) (pi\<bullet>t) (T\<^isub>1\<rightarrow>T\<^isub>2)" by (simp)
+    qed
+  next
+    case (QAT_One \<Gamma> s t)
+    then show "\<forall>c (pi::name prm). P1 c (pi\<bullet>\<Gamma>) (pi\<bullet>s) (pi\<bullet>t) TUnit"
+      by (auto intro!: a3 simp add: valid_eqvt)
+  next
+    case (QAP_Var \<Gamma> x T)
+    then show "\<forall>c (pi::name prm). P2 c (pi \<bullet> \<Gamma>) (pi \<bullet> Var x) (pi \<bullet> Var x) T"
+      apply(auto intro!: a4 simp add: valid_eqvt)
+      apply(simp add: set_eqvt[symmetric])
+      apply(perm_simp add: pt_set_bij1a[OF pt_name_inst, OF at_name_inst])
+      done
+  next
+    case (QAP_App \<Gamma> p q T\<^isub>1 T\<^isub>2 s t)
+    then show "\<forall>c (pi::name prm). P2 c (pi\<bullet>\<Gamma>) (pi\<bullet>App p s) (pi\<bullet>App q t) T\<^isub>2"
+      by (auto intro!: a5 simp add: eqvt[simplified])
+  next
+    case (QAP_Const \<Gamma> n)
+    then show "\<forall>c (pi::name prm). P2 c (pi\<bullet>\<Gamma>) (pi\<bullet>Const n) (pi\<bullet>Const n) TBase"
+      by (auto intro!: a6 simp add: eqvt)
+  qed
+  then have "(\<Gamma> \<turnstile> s \<Leftrightarrow> t : T \<longrightarrow> P1 c (([]::name prm)\<bullet>\<Gamma>) (([]::name prm)\<bullet>s) (([]::name prm)\<bullet>t) T) \<and> 
+             (\<Gamma>' \<turnstile> s' \<leftrightarrow> t' : T' \<longrightarrow> P2 c (([]::name prm)\<bullet>\<Gamma>') (([]::name prm)\<bullet>s') (([]::name prm)\<bullet>t') T')"
+    by blast
+  then show ?thesis by simp
+qed
+
+(* post-processing of the strong induction principle proved above; *) 
+(* the code extracts the strong_inducts-version from strong_induct *)
+(*<*)
+setup {*
+  PureThy.add_thmss
+    [(("alg_equiv_alg_path_equiv_strong_inducts",
+      ProjectRule.projects (ProofContext.init (the_context())) [1,2]
+        (thm "alg_equiv_alg_path_equiv_strong_induct")), [])] #> snd
+*}
+(*>*)
+
+lemma alg_equiv_valid:
+  shows  "\<Gamma> \<turnstile> s \<Leftrightarrow> t : T \<Longrightarrow> valid \<Gamma>" and  "\<Gamma> \<turnstile> s \<leftrightarrow> t : T \<Longrightarrow> valid \<Gamma>"
+by (induct rule : alg_equiv_alg_path_equiv.inducts, auto)
+
+text{* \subsubsection{Inversion lemmas for algorithmic term and path equivalences} *}
+
+declare trm.inject  [simp add]
+declare ty.inject  [simp add]
+
+inductive_cases2 whn_inv_auto[elim]: "t \<Down> t'"
+
+inductive_cases2 alg_equiv_Base_inv_auto[elim]: "\<Gamma> \<turnstile> s\<Leftrightarrow>t : TBase"
+inductive_cases2 alg_equiv_Arrow_inv_auto[elim]: "\<Gamma> \<turnstile> s\<Leftrightarrow>t : T\<^isub>1 \<rightarrow> T\<^isub>2"
+
+inductive_cases2 alg_path_equiv_Base_inv_auto[elim]: "\<Gamma> \<turnstile> s\<leftrightarrow>t : TBase"
+inductive_cases2 alg_path_equiv_Unit_inv_auto[elim]: "\<Gamma> \<turnstile> s\<leftrightarrow>t : TUnit"
+inductive_cases2 alg_path_equiv_Arrow_inv_auto[elim]: "\<Gamma> \<turnstile> s\<leftrightarrow>t : T\<^isub>1 \<rightarrow> T\<^isub>2"
+
+inductive_cases2 alg_path_equiv_Var_left_inv_auto[elim]: "\<Gamma> \<turnstile> Var x \<leftrightarrow> t : T"
+inductive_cases2 alg_path_equiv_Var_left_inv_auto'[elim]: "\<Gamma> \<turnstile> Var x \<leftrightarrow> t : T'"
+inductive_cases2 alg_path_equiv_Var_right_inv_auto[elim]: "\<Gamma> \<turnstile> s \<leftrightarrow> Var x : T"
+inductive_cases2 alg_path_equiv_Var_right_inv_auto'[elim]: "\<Gamma> \<turnstile> s \<leftrightarrow> Var x : T'"
+inductive_cases2 alg_path_equiv_Const_left_inv_auto[elim]: "\<Gamma> \<turnstile> Const n \<leftrightarrow> t : T"
+inductive_cases2 alg_path_equiv_Const_right_inv_auto[elim]: "\<Gamma> \<turnstile> s \<leftrightarrow> Const n : T"
+inductive_cases2 alg_path_equiv_App_left_inv_auto[elim]: "\<Gamma> \<turnstile> App p s \<leftrightarrow> t : T"
+inductive_cases2 alg_path_equiv_App_right_inv_auto[elim]: "\<Gamma> \<turnstile> s \<leftrightarrow> App q t : T"
+inductive_cases2 alg_path_equiv_Lam_left_inv_auto[elim]: "\<Gamma> \<turnstile> Lam[x].s \<leftrightarrow> t : T"
+inductive_cases2 alg_path_equiv_Lam_right_inv_auto[elim]: "\<Gamma> \<turnstile> t \<leftrightarrow> Lam[x].s : T"
+
+declare trm.inject [simp del]
+declare ty.inject [simp del]
+
+text {* \section{Completeness of the algorithm} *}
+
+lemma algorithmic_monotonicity:
+  fixes \<Gamma>':: "(name\<times>ty) list"
+  shows "\<Gamma> \<turnstile> s \<Leftrightarrow> t : T \<Longrightarrow> \<Gamma>\<lless>\<Gamma>' \<Longrightarrow> \<Gamma>' \<turnstile> s \<Leftrightarrow> t : T"
+  and "\<Gamma> \<turnstile> s \<leftrightarrow> t : T \<Longrightarrow> \<Gamma>\<lless>\<Gamma>' \<Longrightarrow> \<Gamma>' \<turnstile> s \<leftrightarrow> t : T"
+proof (nominal_induct \<Gamma> s t T and \<Gamma> s t T avoiding: \<Gamma>' rule: alg_equiv_alg_path_equiv_strong_inducts)
+ case (QAT_Arrow x \<Gamma> s t T\<^isub>1 T\<^isub>2 \<Gamma>')
+  have fs:"x\<sharp>\<Gamma>" "x\<sharp>s" "x\<sharp>t" by fact
+  have h2:"\<Gamma>\<lless>\<Gamma>'" by fact
+  have ih:"\<And>\<Gamma>'. \<lbrakk>(x,T\<^isub>1)#\<Gamma> \<lless> \<Gamma>'\<rbrakk>  \<Longrightarrow> \<Gamma>' \<turnstile> App s (Var x) \<Leftrightarrow> App t (Var x) : T\<^isub>2" by fact
+  have "x\<sharp>\<Gamma>'" by fact
+  then have sub:"(x,T\<^isub>1)#\<Gamma> \<lless> (x,T\<^isub>1)#\<Gamma>'" using h2 by auto
+  then have "(x,T\<^isub>1)#\<Gamma>' \<turnstile> App s (Var x) \<Leftrightarrow> App t (Var x) : T\<^isub>2" using ih by auto
+  then show "\<Gamma>' \<turnstile> s \<Leftrightarrow> t : T\<^isub>1\<rightarrow>T\<^isub>2" using sub fs by auto
+qed (auto)
+
+lemma valid_monotonicity[elim]:
+ assumes "\<Gamma> \<lless> \<Gamma>'" and "x\<sharp>\<Gamma>'"
+ shows "(x,T\<^isub>1)#\<Gamma> \<lless> (x,T\<^isub>1)#\<Gamma>'"
+using assms by auto
+
+lemma algorithmic_monotonicity_auto:
+  fixes \<Gamma>':: "(name\<times>ty) list"
+  shows "\<Gamma> \<turnstile> s \<Leftrightarrow> t : T \<Longrightarrow> \<Gamma>\<lless>\<Gamma>' \<Longrightarrow> \<Gamma>' \<turnstile> s \<Leftrightarrow> t : T"
+  and "\<Gamma> \<turnstile> s \<leftrightarrow> t : T \<Longrightarrow> \<Gamma>\<lless>\<Gamma>' \<Longrightarrow> \<Gamma>' \<turnstile> s \<leftrightarrow> t : T"
+by (nominal_induct \<Gamma> s t T and \<Gamma> s t T avoiding: \<Gamma>' rule: alg_equiv_alg_path_equiv_strong_inducts, auto simp add: valid_monotonicity)
  
-lemma fresh_subst_fresh:
-    assumes "a\<sharp>e"
-    shows "a\<sharp>t[a::=e]"
+text {* \subsection{Definition of the logical relation} *}
+
+function log_equiv :: "((name\<times>ty) list \<Rightarrow> trm \<Rightarrow> trm \<Rightarrow> ty \<Rightarrow> bool)"   
+                      ("_ \<turnstile> _ is _ : _" [60,60,60,60] 60) 
+where    
+   "\<Gamma> \<turnstile> s is t : TUnit = valid \<Gamma>"
+ | "\<Gamma> \<turnstile> s is t : TBase = \<Gamma> \<turnstile> s \<Leftrightarrow> t : TBase"
+ | "\<Gamma> \<turnstile> s is t : (T\<^isub>1 \<rightarrow> T\<^isub>2) =  
+           (valid \<Gamma> \<and> (\<forall>\<Gamma>' s' t'. \<Gamma>\<lless>\<Gamma>' \<longrightarrow> \<Gamma>' \<turnstile> s' is t' : T\<^isub>1 \<longrightarrow>  (\<Gamma>' \<turnstile> (App s s') is (App t t') : T\<^isub>2)))"
+apply (auto simp add: ty.inject)
+apply (subgoal_tac "(\<exists>T\<^isub>1 T\<^isub>2. b=T\<^isub>1 \<rightarrow> T\<^isub>2) \<or> b=TUnit \<or> b=TBase" )
+apply (force)
+apply (rule ty_cases)
+done
+
+termination
+apply(relation "measure (\<lambda>(_,_,_,T). size T)")
+apply(auto)
+done
+
+lemma log_equiv_valid: 
+  assumes "\<Gamma> \<turnstile> s is t : T"
+  shows "valid \<Gamma>"
 using assms 
-by (nominal_induct t avoiding: a e rule: trm.induct)
-   (auto simp add: fresh_atm abs_fresh fresh_nat) 
+by (induct rule: log_equiv.induct,auto elim: alg_equiv_valid)
+
+text {* \subsubsection{Monotonicity of the logical equivalence relation} *}
+
+lemma logical_monotonicity :
+ fixes T::ty
+ assumes "\<Gamma> \<turnstile> s is t : T" "\<Gamma>\<lless>\<Gamma>'" 
+ shows "\<Gamma>' \<turnstile> s is t : T"
+using assms
+proof (induct arbitrary: \<Gamma>' rule: log_equiv.induct)
+  case (2 \<Gamma> s t \<Gamma>')
+  then show "\<Gamma>' \<turnstile> s is t : TBase" using algorithmic_monotonicity by auto
+next
+  case (3 \<Gamma> s t T\<^isub>1 T\<^isub>2 \<Gamma>')
+  then show "\<Gamma>' \<turnstile> s is t : T\<^isub>1\<rightarrow>T\<^isub>2" by force 
+qed (auto)
+
+text {* If two terms are path equivalent then they are in normal form. *}
 
 lemma path_equiv_implies_nf:
   assumes "\<Gamma> \<turnstile> s \<leftrightarrow> t : T"
@@ -844,44 +1023,38 @@ lemma path_equiv_implies_nf:
 using assms
 by (induct rule: alg_equiv_alg_path_equiv.inducts(2)) (simp, auto)
 
-lemma path_equiv_implies_nf:
-  shows "\<Gamma> \<turnstile> s <=> t : T \<Longrightarrow> True"
-    and "\<Gamma> \<turnstile> s \<leftrightarrow> t : T \<Longrightarrow> s \<leadsto>|"
-        "\<Gamma> \<turnstile> s \<leftrightarrow> t : T \<Longrightarrow> t \<leadsto>|"
-by (induct rule: alg_equiv_alg_path_equiv.inducts) (auto)
-
 lemma main_lemma:
-  shows "\<Gamma> \<turnstile> s is t : T \<Longrightarrow> \<Gamma> \<turnstile> s <=> t : T" and "\<Gamma> \<turnstile> p \<leftrightarrow> q : T \<Longrightarrow> \<Gamma> \<turnstile> p is q : T"
+  shows "\<Gamma> \<turnstile> s is t : T \<Longrightarrow> \<Gamma> \<turnstile> s \<Leftrightarrow> t : T" and "\<Gamma> \<turnstile> p \<leftrightarrow> q : T \<Longrightarrow> \<Gamma> \<turnstile> p is q : T"
 proof (nominal_induct T arbitrary: \<Gamma> s t p q rule:ty.induct)
-  case (Arrow T1 T2)
+  case (Arrow T\<^isub>1 T\<^isub>2)
   { 
     case (1 \<Gamma> s t)
-    have ih1:"\<And>\<Gamma> s t. \<Gamma> \<turnstile> s is t : T2 \<Longrightarrow> \<Gamma> \<turnstile> s <=> t : T2" by fact
-    have ih2:"\<And>\<Gamma> s t. \<Gamma> \<turnstile> s \<leftrightarrow> t : T1 \<Longrightarrow> \<Gamma> \<turnstile> s is t : T1" by fact
-    have h:"\<Gamma> \<turnstile> s is t : T1\<rightarrow>T2" by fact
+    have ih1:"\<And>\<Gamma> s t. \<Gamma> \<turnstile> s is t : T\<^isub>2 \<Longrightarrow> \<Gamma> \<turnstile> s \<Leftrightarrow> t : T\<^isub>2" by fact
+    have ih2:"\<And>\<Gamma> s t. \<Gamma> \<turnstile> s \<leftrightarrow> t : T\<^isub>1 \<Longrightarrow> \<Gamma> \<turnstile> s is t : T\<^isub>1" by fact
+    have h:"\<Gamma> \<turnstile> s is t : T\<^isub>1\<rightarrow>T\<^isub>2" by fact
     obtain x::name where fs:"x\<sharp>(\<Gamma>,s,t)" by (erule exists_fresh[OF fs_name1])
     have "valid \<Gamma>" using h log_equiv_valid by auto
-    then have v:"valid ((x,T1)#\<Gamma>)" using fs by auto
-    then have "(x,T1)#\<Gamma> \<turnstile> Var x \<leftrightarrow> Var x : T1" by auto
-    then have "(x,T1)#\<Gamma> \<turnstile> Var x is Var x : T1" using ih2 by auto
-    then have "(x,T1)#\<Gamma> \<turnstile> App s (Var x) is App t (Var x) : T2" using h v by auto
-    then have "(x,T1)#\<Gamma> \<turnstile> App s (Var x) <=> App t (Var x) : T2" using ih1 by auto
-    then show "\<Gamma> \<turnstile> s <=> t : T1\<rightarrow>T2" using fs by (auto simp add: fresh_prod)
+    then have v:"valid ((x,T\<^isub>1)#\<Gamma>)" using fs by auto
+    then have "(x,T\<^isub>1)#\<Gamma> \<turnstile> Var x \<leftrightarrow> Var x : T\<^isub>1" by auto
+    then have "(x,T\<^isub>1)#\<Gamma> \<turnstile> Var x is Var x : T\<^isub>1" using ih2 by auto
+    then have "(x,T\<^isub>1)#\<Gamma> \<turnstile> App s (Var x) is App t (Var x) : T\<^isub>2" using h v by auto
+    then have "(x,T\<^isub>1)#\<Gamma> \<turnstile> App s (Var x) \<Leftrightarrow> App t (Var x) : T\<^isub>2" using ih1 by auto
+    then show "\<Gamma> \<turnstile> s \<Leftrightarrow> t : T\<^isub>1\<rightarrow>T\<^isub>2" using fs by (auto simp add: fresh_prod)
   next
     case (2 \<Gamma> p q)
-    have h:"\<Gamma> \<turnstile> p \<leftrightarrow> q : T1\<rightarrow>T2" by fact
-    have ih1:"\<And>\<Gamma> s t. \<Gamma> \<turnstile> s \<leftrightarrow> t : T2 \<Longrightarrow> \<Gamma> \<turnstile> s is t : T2" by fact
-    have ih2:"\<And>\<Gamma> s t. \<Gamma> \<turnstile> s is t : T1 \<Longrightarrow> \<Gamma> \<turnstile> s <=> t : T1" by fact
+    have h:"\<Gamma> \<turnstile> p \<leftrightarrow> q : T\<^isub>1\<rightarrow>T\<^isub>2" by fact
+    have ih1:"\<And>\<Gamma> s t. \<Gamma> \<turnstile> s \<leftrightarrow> t : T\<^isub>2 \<Longrightarrow> \<Gamma> \<turnstile> s is t : T\<^isub>2" by fact
+    have ih2:"\<And>\<Gamma> s t. \<Gamma> \<turnstile> s is t : T\<^isub>1 \<Longrightarrow> \<Gamma> \<turnstile> s \<Leftrightarrow> t : T\<^isub>1" by fact
     {
       fix \<Gamma>' s t
-      assume "\<Gamma>\<lless>\<Gamma>'" and hl:"\<Gamma>' \<turnstile> s is t : T1"
-      then have "\<Gamma>' \<turnstile> p \<leftrightarrow> q : T1 \<rightarrow> T2" using h algorithmic_monotonicity by auto
-      moreover have "\<Gamma>' \<turnstile> s <=> t : T1" using ih2 hl by auto
-      ultimately have "\<Gamma>' \<turnstile> App p s \<leftrightarrow> App q t : T2" by auto
-      then have "\<Gamma>' \<turnstile> App p s is App q t : T2" using ih1 by auto
+      assume "\<Gamma>\<lless>\<Gamma>'" and hl:"\<Gamma>' \<turnstile> s is t : T\<^isub>1"
+      then have "\<Gamma>' \<turnstile> p \<leftrightarrow> q : T\<^isub>1 \<rightarrow> T\<^isub>2" using h algorithmic_monotonicity by auto
+      moreover have "\<Gamma>' \<turnstile> s \<Leftrightarrow> t : T\<^isub>1" using ih2 hl by auto
+      ultimately have "\<Gamma>' \<turnstile> App p s \<leftrightarrow> App q t : T\<^isub>2" by auto
+      then have "\<Gamma>' \<turnstile> App p s is App q t : T\<^isub>2" using ih1 by auto
     }
     moreover have "valid \<Gamma>" using h alg_equiv_valid by auto
-    ultimately show "\<Gamma> \<turnstile> p is q : T1\<rightarrow>T2"  by auto
+    ultimately show "\<Gamma> \<turnstile> p is q : T\<^isub>1\<rightarrow>T\<^isub>2"  by auto
   }
 next
   case TBase
@@ -889,30 +1062,20 @@ next
     have h:"\<Gamma> \<turnstile> s \<leftrightarrow> t : TBase" by fact
     then have "s \<leadsto>|" and "t \<leadsto>|" using path_equiv_implies_nf by auto
     then have "s \<Down> s" and "t \<Down> t" by auto
-    then have "\<Gamma> \<turnstile> s <=> t : TBase" using h by auto
+    then have "\<Gamma> \<turnstile> s \<Leftrightarrow> t : TBase" using h by auto
     then show "\<Gamma> \<turnstile> s is t : TBase" by auto
   }
 qed (auto elim:alg_equiv_valid)
 
 corollary corollary_main:
   assumes a: "\<Gamma> \<turnstile> s \<leftrightarrow> t : T"
-  shows "\<Gamma> \<turnstile> s <=> t : T"
+  shows "\<Gamma> \<turnstile> s \<Leftrightarrow> t : T"
 using a main_lemma by blast
 
-lemma algorithmic_symmetry_aux:
-  shows "\<Gamma> \<turnstile> s <=> t : T \<Longrightarrow> \<Gamma> \<turnstile> t <=> s : T" 
+lemma algorithmic_symmetry:
+  shows "\<Gamma> \<turnstile> s \<Leftrightarrow> t : T \<Longrightarrow> \<Gamma> \<turnstile> t \<Leftrightarrow> s : T" 
   and   "\<Gamma> \<turnstile> s \<leftrightarrow> t : T \<Longrightarrow> \<Gamma> \<turnstile> t \<leftrightarrow> s : T"
 by (induct rule: alg_equiv_alg_path_equiv.inducts) (auto)
-
-lemma algorithmic_symmetry:
-  assumes a: "\<Gamma> \<turnstile> s <=> t : T"
-  shows "\<Gamma> \<turnstile> t <=> s : T"
-using a by (simp add: algorithmic_symmetry_aux)
-
-lemma algorithmic_path_symmetry:
-  assumes a: "\<Gamma> \<turnstile> s \<leftrightarrow> t : T"
-  shows "\<Gamma> \<turnstile> t \<leftrightarrow> s : T"
-using a by (simp add: algorithmic_symmetry_aux)
 
 lemma red_unicity : 
   assumes a: "x \<leadsto> a" 
@@ -943,72 +1106,49 @@ proof (induct arbitrary: b)
   then show "a=b" using ih hl by auto
 qed (auto)
 
-lemma Q_eqvt :
-  fixes pi:: "name prm"
-  shows "\<Gamma> \<turnstile> s <=> t : T \<Longrightarrow> (pi\<bullet>\<Gamma>) \<turnstile> (pi\<bullet>s) <=> (pi\<bullet>t) : T"
-  and "\<Gamma> \<turnstile> s \<leftrightarrow> t : T \<Longrightarrow> (pi\<bullet>\<Gamma>) \<turnstile> (pi\<bullet>s) \<leftrightarrow> (pi\<bullet>t) : T"
-using assms
-proof (induct rule:alg_equiv_alg_path_equiv.inducts)
-  case (QAP_Var \<Gamma> x T)
-  then have "pi\<bullet>(x,T) \<in> (pi\<bullet>(set \<Gamma>))" using in_eqvt by blast
-  then have "(pi\<bullet>x,T) \<in> (set (pi\<bullet>\<Gamma>))" using set_eqvt perm_ty by auto
-  moreover have "valid \<Gamma>" by fact
-  ultimately show ?case using valid_eqvt by auto
-next
-  case (QAT_Arrow x \<Gamma> s t T1 T2)
-  then have h:"((pi\<bullet>x)\<sharp>(pi\<bullet>\<Gamma>))" "((pi\<bullet>x)\<sharp>(pi\<bullet>s))" "((pi\<bullet>x)\<sharp>(pi\<bullet>t))"  using fresh_bij by auto
-  have "(pi\<bullet>((x,T1)#\<Gamma>)) \<turnstile> pi \<bullet> (App s (Var x)) <=> pi \<bullet> (App t (Var x)) : T2" by fact
-  then have "(pi\<bullet>((x,T1)#\<Gamma>)) \<turnstile> (App (pi\<bullet>s) (Var (pi\<bullet>x))) <=> (App (pi\<bullet>t) (Var (pi\<bullet>x))) : T2" by auto
-  moreover have "pi\<bullet>((x,T1)#\<Gamma>) = (pi\<bullet>x,pi\<bullet>T1)#(pi\<bullet>\<Gamma>)" by auto
-  ultimately have "((pi\<bullet>x,T1)#(pi\<bullet>\<Gamma>))  \<turnstile> (App (pi\<bullet>s) (Var (pi\<bullet>x))) <=> (App (pi\<bullet>t) (Var (pi\<bullet>x))) : T2" 
-    using perm_ty by auto
-  then show ?case using h by auto
-qed (auto elim:whn_eqvt valid_eqvt)
- 
-(* FIXME this lemma should not be here I am reinventing the wheel I guess *)
+nominal_inductive alg_equiv
 
+(* FIXME this lemma should not be here I am reinventing the wheel I guess *)
+(*<*)
 lemma perm_basic[simp]:
  fixes x y::"name"
 shows "[(x,y)]\<bullet>y = x"
 using assms using calc_atm by perm_simp
+(*>*)
+
+text{* \subsection{Strong inversion lemma for algorithmic equivalence} *}
 
 lemma Q_Arrow_strong_inversion:
-  assumes fs:"x\<sharp>\<Gamma>" "x\<sharp>t" "x\<sharp>u" and h:"\<Gamma> \<turnstile> t <=> u : T1\<rightarrow>T2"
-  shows "(x,T1)#\<Gamma> \<turnstile> App t (Var x) <=> App u (Var x) : T2"
+  assumes fs:"x\<sharp>\<Gamma>" "x\<sharp>t" "x\<sharp>u" and h:"\<Gamma> \<turnstile> t \<Leftrightarrow> u : T\<^isub>1\<rightarrow>T\<^isub>2"
+  shows "(x,T\<^isub>1)#\<Gamma> \<turnstile> App t (Var x) \<Leftrightarrow> App u (Var x) : T\<^isub>2"
 proof -
-  obtain y where  fs2:"y\<sharp>\<Gamma>" "y\<sharp>u" "y\<sharp>t" and "(y,T1)#\<Gamma> \<turnstile> App t (Var y) <=> App u (Var y) : T2" 
+  obtain y where  fs2:"y\<sharp>\<Gamma>" "y\<sharp>u" "y\<sharp>t" and "(y,T\<^isub>1)#\<Gamma> \<turnstile> App t (Var y) \<Leftrightarrow> App u (Var y) : T\<^isub>2" 
     using h by auto
-  then have "([(x,y)]\<bullet>((y,T1)#\<Gamma>)) \<turnstile> [(x,y)]\<bullet> App t (Var y) <=> [(x,y)]\<bullet> App u (Var y) : T2" 
-    using Q_eqvt by blast
+  then have "([(x,y)]\<bullet>((y,T\<^isub>1)#\<Gamma>)) \<turnstile> [(x,y)]\<bullet> App t (Var y) \<Leftrightarrow> [(x,y)]\<bullet> App u (Var y) : T\<^isub>2" 
+    using  alg_equiv_eqvt[simplified] by blast
   then show ?thesis using fs fs2 by (perm_simp)
 qed
 
-lemma fresh_context: 
-  fixes  \<Gamma> :: "(name\<times>ty) list"
-  and    a :: "name"
-  assumes "a\<sharp>\<Gamma>"
-  shows "\<not>(\<exists>\<tau>::ty. (a,\<tau>)\<in>set \<Gamma>)"
-using assms by(induct \<Gamma>, auto simp add: fresh_prod fresh_list_cons fresh_atm)
+text{* 
+For the \texttt{algorithmic\_transitivity} lemma we need a unicity property.
+But one has to be cautious, because this unicity property is true only for algorithmic path. 
+Indeed the following lemma is \textbf{false}:\\
+\begin{center}
+@{prop "\<lbrakk> \<Gamma> \<turnstile> s \<Leftrightarrow> t : T ; \<Gamma> \<turnstile> s \<Leftrightarrow> u : T' \<rbrakk> \<Longrightarrow> T = T'"}
+\end{center}
+Here is the counter example :\\
+\begin{center}
+@{prop "\<Gamma> \<turnstile> Const n \<Leftrightarrow> Const n : Tbase"} and @{prop "\<Gamma> \<turnstile> Const n \<Leftrightarrow> Const n : TUnit"}
+\end{center}
+*}
 
-lemma type_unicity_in_context:
-  fixes  \<Gamma> :: "(name\<times>ty)list"
-  and    pi:: "name prm"
-  and    a :: "name"
-  and    \<tau> :: "ty"
-  assumes "valid \<Gamma>" and "(x,T1) \<in> set \<Gamma>" and "(x,T2) \<in> set \<Gamma>"
-  shows "T1=T2"
-using assms by (induct \<Gamma>, auto dest!: fresh_context)
-
-(* 
-
-Warning: This lemma is false.
-
+(*
 lemma algorithmic_type_unicity:
-  shows "\<lbrakk> \<Gamma> \<turnstile> s <=> t : T ; \<Gamma> \<turnstile> s <=> u : T' \<rbrakk> \<Longrightarrow> T = T'"
+  shows "\<lbrakk> \<Gamma> \<turnstile> s \<Leftrightarrow> t : T ; \<Gamma> \<turnstile> s \<Leftrightarrow> u : T' \<rbrakk> \<Longrightarrow> T = T'"
   and "\<lbrakk> \<Gamma> \<turnstile> s \<leftrightarrow> t : T ; \<Gamma> \<turnstile> s \<leftrightarrow> u : T' \<rbrakk> \<Longrightarrow> T = T'"
 
 Here is the counter example : 
-\<Gamma> \<turnstile> Const n <=> Const n : Tbase and \<Gamma> \<turnstile> Const n <=> Const n : TUnit
+\<Gamma> \<turnstile> Const n \<Leftrightarrow> Const n : Tbase and \<Gamma> \<turnstile> Const n \<Leftrightarrow> Const n : TUnit
 
 *)
 
@@ -1022,56 +1162,56 @@ proof (induct arbitrary:  u T'
   moreover have "valid \<Gamma>" "(x,T) \<in> set \<Gamma>" by fact
   ultimately show "T=T'" using type_unicity_in_context by auto
 next
-  case (QAP_App \<Gamma> p q T1 T2 s t u T2')
-  have ih:"\<And>u T. \<Gamma> \<turnstile> p \<leftrightarrow> u : T \<Longrightarrow> T1\<rightarrow>T2 = T" by fact
-  have "\<Gamma> \<turnstile> App p s \<leftrightarrow> u : T2'" by fact
-  then obtain r t T1' where "u = App r t"  "\<Gamma> \<turnstile> p \<leftrightarrow> r : T1' \<rightarrow> T2'" by auto
-  then have "T1\<rightarrow>T2 = T1' \<rightarrow> T2'" by auto
-  then show "T2=T2'" using ty.inject by auto
+  case (QAP_App \<Gamma> p q T\<^isub>1 T\<^isub>2 s t u T\<^isub>2')
+  have ih:"\<And>u T. \<Gamma> \<turnstile> p \<leftrightarrow> u : T \<Longrightarrow> T\<^isub>1\<rightarrow>T\<^isub>2 = T" by fact
+  have "\<Gamma> \<turnstile> App p s \<leftrightarrow> u : T\<^isub>2'" by fact
+  then obtain r t T\<^isub>1' where "u = App r t"  "\<Gamma> \<turnstile> p \<leftrightarrow> r : T\<^isub>1' \<rightarrow> T\<^isub>2'" by auto
+  then have "T\<^isub>1\<rightarrow>T\<^isub>2 = T\<^isub>1' \<rightarrow> T\<^isub>2'" by auto
+  then show "T\<^isub>2=T\<^isub>2'" using ty.inject by auto
 qed (auto)
 
 lemma algorithmic_transitivity:
-  shows "\<lbrakk> \<Gamma> \<turnstile> s <=> t : T ; \<Gamma> \<turnstile> t <=> u : T \<rbrakk> \<Longrightarrow> \<Gamma> \<turnstile> s <=> u : T"
+  shows "\<lbrakk> \<Gamma> \<turnstile> s \<Leftrightarrow> t : T ; \<Gamma> \<turnstile> t \<Leftrightarrow> u : T \<rbrakk> \<Longrightarrow> \<Gamma> \<turnstile> s \<Leftrightarrow> u : T"
   and  "\<lbrakk> \<Gamma> \<turnstile> s \<leftrightarrow> t : T ; \<Gamma> \<turnstile> t \<leftrightarrow> u : T \<rbrakk> \<Longrightarrow> \<Gamma> \<turnstile> s \<leftrightarrow> u : T"
 proof (nominal_induct \<Gamma> s t T and \<Gamma> s t T avoiding: u rule: alg_equiv_alg_path_equiv_strong_inducts)
   case (QAT_Base s p t q \<Gamma> u)
   have h:"s \<Down> p" "t \<Down> q" by fact
   have ih:"\<And>u. \<Gamma> \<turnstile> q \<leftrightarrow> u : TBase \<Longrightarrow> \<Gamma> \<turnstile> p \<leftrightarrow> u : TBase" by fact
-  have "\<Gamma> \<turnstile> t <=> u : TBase" by fact
+  have "\<Gamma> \<turnstile> t \<Leftrightarrow> u : TBase" by fact
   then obtain r q' where hl:"t \<Down> q'" "u \<Down> r" "\<Gamma> \<turnstile> q' \<leftrightarrow> r : TBase" by auto
   moreover have eq:"q=q'" using nf_unicity hl h by auto
   ultimately have "\<Gamma> \<turnstile> p \<leftrightarrow> r : TBase" using ih by auto
-  then show "\<Gamma> \<turnstile> s <=> u : TBase" using hl h by auto
+  then show "\<Gamma> \<turnstile> s \<Leftrightarrow> u : TBase" using hl h by auto
 next
-  case (QAT_Arrow  x \<Gamma> s t T1 T2 u)
+  case (QAT_Arrow  x \<Gamma> s t T\<^isub>1 T\<^isub>2 u)
   have fs:"x\<sharp>\<Gamma>" "x\<sharp>s" "x\<sharp>t" by fact
-  moreover have h:"\<Gamma> \<turnstile> t <=> u : T1\<rightarrow>T2" by fact
-  moreover then obtain y where "y\<sharp>\<Gamma>" "y\<sharp>t" "y\<sharp>u" and "(y,T1)#\<Gamma> \<turnstile> App t (Var y) <=> App u (Var y) : T2" 
+  moreover have h:"\<Gamma> \<turnstile> t \<Leftrightarrow> u : T\<^isub>1\<rightarrow>T\<^isub>2" by fact
+  moreover then obtain y where "y\<sharp>\<Gamma>" "y\<sharp>t" "y\<sharp>u" and "(y,T\<^isub>1)#\<Gamma> \<turnstile> App t (Var y) \<Leftrightarrow> App u (Var y) : T\<^isub>2" 
     by auto
   moreover have fs2:"x\<sharp>u" by fact
-  ultimately have "(x,T1)#\<Gamma> \<turnstile> App t (Var x) <=> App u (Var x) : T2" using Q_Arrow_strong_inversion by blast
-  moreover have ih:"\<And> v. (x,T1)#\<Gamma> \<turnstile> App t (Var x) <=> v : T2 \<Longrightarrow> (x,T1)#\<Gamma> \<turnstile> App s (Var x) <=> v : T2" 
+  ultimately have "(x,T\<^isub>1)#\<Gamma> \<turnstile> App t (Var x) \<Leftrightarrow> App u (Var x) : T\<^isub>2" using Q_Arrow_strong_inversion by blast
+  moreover have ih:"\<And> v. (x,T\<^isub>1)#\<Gamma> \<turnstile> App t (Var x) \<Leftrightarrow> v : T\<^isub>2 \<Longrightarrow> (x,T\<^isub>1)#\<Gamma> \<turnstile> App s (Var x) \<Leftrightarrow> v : T\<^isub>2" 
     by fact
-  ultimately have "(x,T1)#\<Gamma> \<turnstile> App s (Var x) <=> App u (Var x) : T2" by auto
-  then show "\<Gamma> \<turnstile> s <=> u : T1\<rightarrow>T2" using fs fs2 by auto
+  ultimately have "(x,T\<^isub>1)#\<Gamma> \<turnstile> App s (Var x) \<Leftrightarrow> App u (Var x) : T\<^isub>2" by auto
+  then show "\<Gamma> \<turnstile> s \<Leftrightarrow> u : T\<^isub>1\<rightarrow>T\<^isub>2" using fs fs2 by auto
 next
-  case (QAP_App \<Gamma> p q T1 T2 s t u)
-  have h1:"\<Gamma> \<turnstile> p \<leftrightarrow> q : T1\<rightarrow>T2" by fact
-  have ih1:"\<And>u. \<Gamma> \<turnstile> q \<leftrightarrow> u : T1\<rightarrow>T2 \<Longrightarrow> \<Gamma> \<turnstile> p \<leftrightarrow> u : T1\<rightarrow>T2" by fact
-  have "\<Gamma> \<turnstile> s <=> t : T1" by fact
-  have ih2:"\<And>u. \<Gamma> \<turnstile> t <=> u : T1 \<Longrightarrow> \<Gamma> \<turnstile> s <=> u : T1" by fact
-  have "\<Gamma> \<turnstile> App q t \<leftrightarrow> u : T2" by fact
-  then obtain r T1' v where ha:"\<Gamma> \<turnstile> q \<leftrightarrow> r : T1'\<rightarrow>T2" and hb:"\<Gamma> \<turnstile> t <=> v : T1'" and eq:"u = App r v" 
+  case (QAP_App \<Gamma> p q T\<^isub>1 T\<^isub>2 s t u)
+  have h1:"\<Gamma> \<turnstile> p \<leftrightarrow> q : T\<^isub>1\<rightarrow>T\<^isub>2" by fact
+  have ih1:"\<And>u. \<Gamma> \<turnstile> q \<leftrightarrow> u : T\<^isub>1\<rightarrow>T\<^isub>2 \<Longrightarrow> \<Gamma> \<turnstile> p \<leftrightarrow> u : T\<^isub>1\<rightarrow>T\<^isub>2" by fact
+  have "\<Gamma> \<turnstile> s \<Leftrightarrow> t : T\<^isub>1" by fact
+  have ih2:"\<And>u. \<Gamma> \<turnstile> t \<Leftrightarrow> u : T\<^isub>1 \<Longrightarrow> \<Gamma> \<turnstile> s \<Leftrightarrow> u : T\<^isub>1" by fact
+  have "\<Gamma> \<turnstile> App q t \<leftrightarrow> u : T\<^isub>2" by fact
+  then obtain r T\<^isub>1' v where ha:"\<Gamma> \<turnstile> q \<leftrightarrow> r : T\<^isub>1'\<rightarrow>T\<^isub>2" and hb:"\<Gamma> \<turnstile> t \<Leftrightarrow> v : T\<^isub>1'" and eq:"u = App r v" 
     by auto
-  moreover have "\<Gamma> \<turnstile> q \<leftrightarrow> p : T1\<rightarrow>T2" using h1 algorithmic_path_symmetry by auto
-  ultimately have "T1'\<rightarrow>T2 = T1\<rightarrow>T2" using algorithmic_path_type_unicity by auto
-  then have "T1' = T1" using ty.inject by auto
-  then have "\<Gamma> \<turnstile> s <=> v : T1" "\<Gamma> \<turnstile> p \<leftrightarrow> r : T1\<rightarrow>T2" using ih1 ih2 ha hb by auto
-  then show "\<Gamma> \<turnstile> App p s \<leftrightarrow> u : T2" using eq by auto
+  moreover have "\<Gamma> \<turnstile> q \<leftrightarrow> p : T\<^isub>1\<rightarrow>T\<^isub>2" using h1 algorithmic_symmetry by auto
+  ultimately have "T\<^isub>1'\<rightarrow>T\<^isub>2 = T\<^isub>1\<rightarrow>T\<^isub>2" using algorithmic_path_type_unicity by auto
+  then have "T\<^isub>1' = T\<^isub>1" using ty.inject by auto
+  then have "\<Gamma> \<turnstile> s \<Leftrightarrow> v : T\<^isub>1" "\<Gamma> \<turnstile> p \<leftrightarrow> r : T\<^isub>1\<rightarrow>T\<^isub>2" using ih1 ih2 ha hb by auto
+  then show "\<Gamma> \<turnstile> App p s \<leftrightarrow> u : T\<^isub>2" using eq by auto
 qed (auto)
 
 lemma algorithmic_weak_head_closure:
-  shows "\<lbrakk>\<Gamma> \<turnstile> s <=> t : T ; s' \<leadsto> s; t' \<leadsto> t\<rbrakk> \<Longrightarrow> \<Gamma> \<turnstile> s' <=> t' : T"
+  shows "\<lbrakk>\<Gamma> \<turnstile> s \<Leftrightarrow> t : T ; s' \<leadsto> s; t' \<leadsto> t\<rbrakk> \<Longrightarrow> \<Gamma> \<turnstile> s' \<Leftrightarrow> t' : T"
 by (nominal_induct \<Gamma> s t T avoiding: s' t'  
     rule: alg_equiv_alg_path_equiv_strong_inducts(1) [of _ _ _ _ "%a b c d e. True"])
    (auto)
@@ -1090,32 +1230,29 @@ proof (nominal_induct arbitrary: \<Gamma> s t u  rule:ty.induct)
   case TBase
   then show "\<Gamma> \<turnstile> s is u : TBase" by (auto elim:  algorithmic_transitivity)
 next 
-  case (Arrow T1 T2 \<Gamma> s t u)
-  have h1:"\<Gamma> \<turnstile> s is t : T1 \<rightarrow> T2" by fact
-  have h2:"\<Gamma> \<turnstile> t is u : T1 \<rightarrow> T2" by fact
-  have ih1:"\<And>\<Gamma> s t u. \<lbrakk>\<Gamma> \<turnstile> s is t : T1; \<Gamma> \<turnstile> t is u : T1\<rbrakk> \<Longrightarrow> \<Gamma> \<turnstile> s is u : T1" by fact
-  have ih2:"\<And>\<Gamma> s t u. \<lbrakk>\<Gamma> \<turnstile> s is t : T2; \<Gamma> \<turnstile> t is u : T2\<rbrakk> \<Longrightarrow> \<Gamma> \<turnstile> s is u : T2" by fact
+  case (Arrow T\<^isub>1 T\<^isub>2 \<Gamma> s t u)
+  have h1:"\<Gamma> \<turnstile> s is t : T\<^isub>1 \<rightarrow> T\<^isub>2" by fact
+  have h2:"\<Gamma> \<turnstile> t is u : T\<^isub>1 \<rightarrow> T\<^isub>2" by fact
+  have ih1:"\<And>\<Gamma> s t u. \<lbrakk>\<Gamma> \<turnstile> s is t : T\<^isub>1; \<Gamma> \<turnstile> t is u : T\<^isub>1\<rbrakk> \<Longrightarrow> \<Gamma> \<turnstile> s is u : T\<^isub>1" by fact
+  have ih2:"\<And>\<Gamma> s t u. \<lbrakk>\<Gamma> \<turnstile> s is t : T\<^isub>2; \<Gamma> \<turnstile> t is u : T\<^isub>2\<rbrakk> \<Longrightarrow> \<Gamma> \<turnstile> s is u : T\<^isub>2" by fact
   {
     fix \<Gamma>' s' u'
-    assume hsub:"\<Gamma>\<lless>\<Gamma>'" and hl:"\<Gamma>' \<turnstile> s' is u' : T1"
-    then have "\<Gamma>' \<turnstile> u' is s' : T1" using logical_symmetry by blast
-    then have "\<Gamma>' \<turnstile> u' is u' : T1" using ih1 hl by blast
-    then have "\<Gamma>' \<turnstile> App t u' is App u u' : T2" using h2 hsub by auto
-    moreover have "\<Gamma>' \<turnstile>  App s s' is App t u' : T2" using h1 hsub hl by auto
-    ultimately have "\<Gamma>' \<turnstile>  App s s' is App u u' : T2" using ih2 by blast
+    assume hsub:"\<Gamma>\<lless>\<Gamma>'" and hl:"\<Gamma>' \<turnstile> s' is u' : T\<^isub>1"
+    then have "\<Gamma>' \<turnstile> u' is s' : T\<^isub>1" using logical_symmetry by blast
+    then have "\<Gamma>' \<turnstile> u' is u' : T\<^isub>1" using ih1 hl by blast
+    then have "\<Gamma>' \<turnstile> App t u' is App u u' : T\<^isub>2" using h2 hsub by auto
+    moreover have "\<Gamma>' \<turnstile>  App s s' is App t u' : T\<^isub>2" using h1 hsub hl by auto
+    ultimately have "\<Gamma>' \<turnstile>  App s s' is App u u' : T\<^isub>2" using ih2 by blast
   }
   moreover have "valid \<Gamma>" using h1 alg_equiv_valid by auto
-  ultimately show "\<Gamma> \<turnstile> s is u : T1 \<rightarrow> T2" by auto
+  ultimately show "\<Gamma> \<turnstile> s is u : T\<^isub>1 \<rightarrow> T\<^isub>2" by auto
 qed (auto)
 
 lemma logical_weak_head_closure:
-  assumes a: "\<Gamma> \<turnstile> s is t : T" "s' \<leadsto> s" "t' \<leadsto> t"
+  assumes "\<Gamma> \<turnstile> s is t : T" "s' \<leadsto> s" "t' \<leadsto> t"
   shows "\<Gamma> \<turnstile> s' is t' : T"
-using a
-apply(nominal_induct arbitrary: \<Gamma> s t s' t' rule:ty.induct)
-apply(auto simp add: algorithmic_weak_head_closure)
-apply(blast)
-done
+using assms algorithmic_weak_head_closure 
+by (nominal_induct arbitrary: \<Gamma> s t s' t' rule:ty.induct) (auto, blast)
 
 lemma logical_weak_head_closure':
   assumes "\<Gamma> \<turnstile> s is t : T" "s' \<leadsto> s" 
@@ -1127,22 +1264,22 @@ proof (nominal_induct arbitrary: \<Gamma> s t s' rule: ty.induct)
 next
   case (TUnit \<Gamma> s t s')
   then show ?case by auto
-next
-  case (Arrow T1 T2 \<Gamma> s t s')
+next 
+  case (Arrow T\<^isub>1 T\<^isub>2 \<Gamma> s t s')
   have h1:"s' \<leadsto> s" by fact
-  have ih:"\<And>\<Gamma> s t s'. \<lbrakk>\<Gamma> \<turnstile> s is t : T2; s' \<leadsto> s\<rbrakk> \<Longrightarrow> \<Gamma> \<turnstile> s' is t : T2" by fact
-  have h2:"\<Gamma> \<turnstile> s is t : T1\<rightarrow>T2" by fact
-  then have hb:"\<forall>\<Gamma>' s' t'. \<Gamma>\<lless>\<Gamma>' \<longrightarrow> \<Gamma>' \<turnstile> s' is t' : T1 \<longrightarrow>  (\<Gamma>' \<turnstile> (App s s') is (App t t') : T2)" by auto
+  have ih:"\<And>\<Gamma> s t s'. \<lbrakk>\<Gamma> \<turnstile> s is t : T\<^isub>2; s' \<leadsto> s\<rbrakk> \<Longrightarrow> \<Gamma> \<turnstile> s' is t : T\<^isub>2" by fact
+  have h2:"\<Gamma> \<turnstile> s is t : T\<^isub>1\<rightarrow>T\<^isub>2" by fact
+  then have hb:"\<forall>\<Gamma>' s' t'. \<Gamma>\<lless>\<Gamma>' \<longrightarrow> \<Gamma>' \<turnstile> s' is t' : T\<^isub>1 \<longrightarrow>  (\<Gamma>' \<turnstile> (App s s') is (App t t') : T\<^isub>2)" by auto
   {
-    fix \<Gamma>' s2 t2
-    assume "\<Gamma>\<lless>\<Gamma>'" and "\<Gamma>' \<turnstile> s2 is t2 : T1"
-    then have "\<Gamma>' \<turnstile> (App s s2) is (App t t2) : T2" using hb by auto
-    moreover have "(App s' s2)  \<leadsto> (App s s2)" using h1 by auto  
-    ultimately have "\<Gamma>' \<turnstile> App s' s2 is App t t2 : T2" using ih by auto
+    fix \<Gamma>' s\<^isub>2 t\<^isub>2
+    assume "\<Gamma>\<lless>\<Gamma>'" and "\<Gamma>' \<turnstile> s\<^isub>2 is t\<^isub>2 : T\<^isub>1"
+    then have "\<Gamma>' \<turnstile> (App s s\<^isub>2) is (App t t\<^isub>2) : T\<^isub>2" using hb by auto
+    moreover have "(App s' s\<^isub>2)  \<leadsto> (App s s\<^isub>2)" using h1 by auto  
+    ultimately have "\<Gamma>' \<turnstile> App s' s\<^isub>2 is App t t\<^isub>2 : T\<^isub>2" using ih by auto
   }
   moreover have "valid \<Gamma>" using h2 log_equiv_valid by auto
-  ultimately show "\<Gamma> \<turnstile> s' is t : T1\<rightarrow>T2" by auto
-qed
+  ultimately show "\<Gamma> \<turnstile> s' is t : T\<^isub>1\<rightarrow>T\<^isub>2" by auto
+qed 
 
 abbreviation 
  log_equiv_subst :: "(name\<times>ty) list \<Rightarrow> (name\<times>trm) list \<Rightarrow>  (name\<times>trm) list \<Rightarrow> (name\<times>ty) list \<Rightarrow> bool"  
@@ -1200,28 +1337,28 @@ theorem fundamental_theorem:
   shows "\<Gamma>' \<turnstile> \<gamma><t> is \<theta><t> : T"   
 using assms
 proof (nominal_induct avoiding:\<Gamma>' \<gamma> \<theta>  rule: typing_induct_strong)
-case (t_Lam x \<Gamma> T1 t2 T2 \<Gamma>' \<gamma> \<theta>)
+case (t_Lam x \<Gamma> T\<^isub>1 t\<^isub>2 T\<^isub>2 \<Gamma>' \<gamma> \<theta>)
 have fs:"x\<sharp>\<gamma>" "x\<sharp>\<theta>" "x\<sharp>\<Gamma>" by fact
 have h:"\<Gamma>' \<turnstile> \<gamma> is \<theta> over \<Gamma>" by fact
-have ih:"\<And> \<Gamma>' \<gamma> \<theta>. \<Gamma>' \<turnstile> \<gamma> is \<theta> over (x,T1)#\<Gamma> \<Longrightarrow> \<Gamma>' \<turnstile> \<gamma><t2> is \<theta><t2> : T2" by fact
+have ih:"\<And> \<Gamma>' \<gamma> \<theta>. \<Gamma>' \<turnstile> \<gamma> is \<theta> over (x,T\<^isub>1)#\<Gamma> \<Longrightarrow> \<Gamma>' \<turnstile> \<gamma><t\<^isub>2> is \<theta><t\<^isub>2> : T\<^isub>2" by fact
 {
   fix \<Gamma>'' s' t'
-  assume "\<Gamma>'\<lless>\<Gamma>''" and hl:"\<Gamma>''\<turnstile> s' is t' : T1"
+  assume "\<Gamma>'\<lless>\<Gamma>''" and hl:"\<Gamma>''\<turnstile> s' is t' : T\<^isub>1"
   then have "\<Gamma>'' \<turnstile> \<gamma> is \<theta> over \<Gamma>" using logical_subst_monotonicity h by blast
-  then have "\<Gamma>'' \<turnstile> (x,s')#\<gamma> is (x,t')#\<theta> over (x,T1)#\<Gamma>" using equiv_subst_ext hl fs by blast
-  then have "\<Gamma>'' \<turnstile> (x,s')#\<gamma><t2> is (x,t')#\<theta><t2> : T2" using ih by auto
-  then have "\<Gamma>''\<turnstile>\<gamma><t2>[x::=s'] is \<theta><t2>[x::=t'] : T2" using psubst_subst_psubst fs by simp
-  moreover have "App (Lam [x].\<gamma><t2>) s' \<leadsto> \<gamma><t2>[x::=s']" by auto
-  moreover have "App (Lam [x].\<theta><t2>) t' \<leadsto> \<theta><t2>[x::=t']" by auto
-  ultimately have "\<Gamma>''\<turnstile> App (Lam [x].\<gamma><t2>) s' is App (Lam [x].\<theta><t2>) t' : T2" 
+  then have "\<Gamma>'' \<turnstile> (x,s')#\<gamma> is (x,t')#\<theta> over (x,T\<^isub>1)#\<Gamma>" using equiv_subst_ext hl fs by blast
+  then have "\<Gamma>'' \<turnstile> (x,s')#\<gamma><t\<^isub>2> is (x,t')#\<theta><t\<^isub>2> : T\<^isub>2" using ih by auto
+  then have "\<Gamma>''\<turnstile>\<gamma><t\<^isub>2>[x::=s'] is \<theta><t\<^isub>2>[x::=t'] : T\<^isub>2" using psubst_subst_psubst fs by simp
+  moreover have "App (Lam [x].\<gamma><t\<^isub>2>) s' \<leadsto> \<gamma><t\<^isub>2>[x::=s']" by auto
+  moreover have "App (Lam [x].\<theta><t\<^isub>2>) t' \<leadsto> \<theta><t\<^isub>2>[x::=t']" by auto
+  ultimately have "\<Gamma>''\<turnstile> App (Lam [x].\<gamma><t\<^isub>2>) s' is App (Lam [x].\<theta><t\<^isub>2>) t' : T\<^isub>2" 
     using logical_weak_head_closure by auto
 }
 moreover have "valid \<Gamma>'" using h by auto
-ultimately show "\<Gamma>' \<turnstile> \<gamma><Lam [x].t2> is \<theta><Lam [x].t2> : T1\<rightarrow>T2" using fs by auto 
+ultimately show "\<Gamma>' \<turnstile> \<gamma><Lam [x].t\<^isub>2> is \<theta><Lam [x].t\<^isub>2> : T\<^isub>1\<rightarrow>T\<^isub>2" using fs by auto 
 qed (auto)
 
 theorem fundamental_theorem_2:
-  assumes h1: "\<Gamma> \<turnstile> s == t : T" 
+  assumes h1: "\<Gamma> \<turnstile> s \<equiv> t : T" 
   and     h2: "\<Gamma>' \<turnstile> \<gamma> is \<theta> over \<Gamma>"
   shows "\<Gamma>' \<turnstile> \<gamma><s> is \<theta><t> : T"
 using h1 h2
@@ -1245,69 +1382,70 @@ next
   moreover have "\<Gamma>' \<turnstile> \<gamma><s> is \<theta><t> : T" using ih1 h by auto
   ultimately show "\<Gamma>' \<turnstile> \<gamma><s> is \<theta><u> : T" using logical_transitivity by blast
 next
-  case (Q_Abs x \<Gamma> T1 s2 t2 T2 \<Gamma>' \<gamma> \<theta>)
+  case (Q_Abs x \<Gamma> T\<^isub>1 s\<^isub>2 t\<^isub>2 T\<^isub>2 \<Gamma>' \<gamma> \<theta>)
   have fs:"x\<sharp>\<Gamma>" by fact
   have fs2: "x\<sharp>\<gamma>" "x\<sharp>\<theta>" by fact 
   have h2:"\<Gamma>' \<turnstile> \<gamma> is \<theta> over \<Gamma>" by fact
-  have ih:"\<And>\<Gamma>' \<gamma> \<theta>. \<Gamma>' \<turnstile> \<gamma> is \<theta> over (x,T1)#\<Gamma> \<Longrightarrow> \<Gamma>' \<turnstile> \<gamma><s2> is \<theta><t2> : T2" by fact
+  have ih:"\<And>\<Gamma>' \<gamma> \<theta>. \<Gamma>' \<turnstile> \<gamma> is \<theta> over (x,T\<^isub>1)#\<Gamma> \<Longrightarrow> \<Gamma>' \<turnstile> \<gamma><s\<^isub>2> is \<theta><t\<^isub>2> : T\<^isub>2" by fact
   {
     fix \<Gamma>'' s' t'
-    assume "\<Gamma>'\<lless>\<Gamma>''" and hl:"\<Gamma>''\<turnstile> s' is t' : T1"
+    assume "\<Gamma>'\<lless>\<Gamma>''" and hl:"\<Gamma>''\<turnstile> s' is t' : T\<^isub>1"
     then have "\<Gamma>'' \<turnstile> \<gamma> is \<theta> over \<Gamma>" using h2 logical_subst_monotonicity by blast
-    then have "\<Gamma>'' \<turnstile> (x,s')#\<gamma> is (x,t')#\<theta> over (x,T1)#\<Gamma>" using equiv_subst_ext hl fs by blast
-    then have "\<Gamma>'' \<turnstile> (x,s')#\<gamma><s2> is (x,t')#\<theta><t2> : T2" using ih by blast
-    then have "\<Gamma>''\<turnstile> \<gamma><s2>[x::=s'] is \<theta><t2>[x::=t'] : T2" using fs2 psubst_subst_psubst by auto
-    moreover have "App (Lam [x]. \<gamma><s2>) s' \<leadsto>  \<gamma><s2>[x::=s']" 
-              and "App (Lam [x].\<theta><t2>) t' \<leadsto> \<theta><t2>[x::=t']" by auto
-    ultimately have "\<Gamma>'' \<turnstile> App (Lam [x]. \<gamma><s2>) s' is App (Lam [x].\<theta><t2>) t' : T2" 
+    then have "\<Gamma>'' \<turnstile> (x,s')#\<gamma> is (x,t')#\<theta> over (x,T\<^isub>1)#\<Gamma>" using equiv_subst_ext hl fs by blast
+    then have "\<Gamma>'' \<turnstile> (x,s')#\<gamma><s\<^isub>2> is (x,t')#\<theta><t\<^isub>2> : T\<^isub>2" using ih by blast
+    then have "\<Gamma>''\<turnstile> \<gamma><s\<^isub>2>[x::=s'] is \<theta><t\<^isub>2>[x::=t'] : T\<^isub>2" using fs2 psubst_subst_psubst by auto
+    moreover have "App (Lam [x]. \<gamma><s\<^isub>2>) s' \<leadsto>  \<gamma><s\<^isub>2>[x::=s']" 
+              and "App (Lam [x].\<theta><t\<^isub>2>) t' \<leadsto> \<theta><t\<^isub>2>[x::=t']" by auto
+    ultimately have "\<Gamma>'' \<turnstile> App (Lam [x]. \<gamma><s\<^isub>2>) s' is App (Lam [x].\<theta><t\<^isub>2>) t' : T\<^isub>2" 
       using logical_weak_head_closure by auto
   }
   moreover have "valid \<Gamma>'" using h2 by auto
-  ultimately have "\<Gamma>' \<turnstile> Lam [x].\<gamma><s2> is Lam [x].\<theta><t2> : T1\<rightarrow>T2" by auto
-  then show "\<Gamma>' \<turnstile> \<gamma><Lam [x].s2> is \<theta><Lam [x].t2> : T1\<rightarrow>T2" using fs2 by auto
+  ultimately have "\<Gamma>' \<turnstile> Lam [x].\<gamma><s\<^isub>2> is Lam [x].\<theta><t\<^isub>2> : T\<^isub>1\<rightarrow>T\<^isub>2" by auto
+  then show "\<Gamma>' \<turnstile> \<gamma><Lam [x].s\<^isub>2> is \<theta><Lam [x].t\<^isub>2> : T\<^isub>1\<rightarrow>T\<^isub>2" using fs2 by auto
 next
-  case (Q_App \<Gamma> s1 t1 T1 T2 s2 t2 \<Gamma>' \<gamma> \<theta>)
-  then show "\<Gamma>' \<turnstile> \<gamma><App s1 s2> is \<theta><App t1 t2> : T2" by auto 
+  case (Q_App \<Gamma> s\<^isub>1 t\<^isub>1 T\<^isub>1 T\<^isub>2 s\<^isub>2 t\<^isub>2 \<Gamma>' \<gamma> \<theta>)
+  then show "\<Gamma>' \<turnstile> \<gamma><App s\<^isub>1 s\<^isub>2> is \<theta><App t\<^isub>1 t\<^isub>2> : T\<^isub>2" by auto 
 next
-  case (Q_Beta x \<Gamma> T1 s12 t12 T2 s2 t2 \<Gamma>' \<gamma> \<theta>)
+  case (Q_Beta x \<Gamma> T\<^isub>1 s12 t12 T\<^isub>2 s\<^isub>2 t\<^isub>2 \<Gamma>' \<gamma> \<theta>)
   have h:"\<Gamma>' \<turnstile> \<gamma> is \<theta> over \<Gamma>" by fact
   have fs:"x\<sharp>\<Gamma>" by fact
   have fs2:"x\<sharp>\<gamma>" "x\<sharp>\<theta>" by fact 
-  have ih1:"\<And>\<Gamma>' \<gamma> \<theta>. \<Gamma>' \<turnstile> \<gamma> is \<theta> over \<Gamma> \<Longrightarrow> \<Gamma>' \<turnstile> \<gamma><s2> is \<theta><t2> : T1" by fact
-  have ih2:"\<And>\<Gamma>' \<gamma> \<theta>. \<Gamma>' \<turnstile> \<gamma> is \<theta> over (x,T1)#\<Gamma> \<Longrightarrow> \<Gamma>' \<turnstile> \<gamma><s12> is \<theta><t12> : T2" by fact
-  have "\<Gamma>' \<turnstile> \<gamma><s2> is \<theta><t2> : T1" using ih1 h by auto
-  then have "\<Gamma>' \<turnstile> (x,\<gamma><s2>)#\<gamma> is (x,\<theta><t2>)#\<theta> over (x,T1)#\<Gamma>" using equiv_subst_ext h fs by blast
-  then have "\<Gamma>' \<turnstile> (x,\<gamma><s2>)#\<gamma><s12> is (x,\<theta><t2>)#\<theta><t12> : T2" using ih2 by auto
-  then have "\<Gamma>' \<turnstile> \<gamma><s12>[x::=\<gamma><s2>] is \<theta><t12>[x::=\<theta><t2>] : T2" using fs2 psubst_subst_psubst by auto
-  then have "\<Gamma>' \<turnstile> \<gamma><s12>[x::=\<gamma><s2>] is \<theta><t12[x::=t2]> : T2" using fs2 psubst_subst_propagate by auto
-  moreover have "App (Lam [x].\<gamma><s12>) (\<gamma><s2>) \<leadsto> \<gamma><s12>[x::=\<gamma><s2>]" by auto 
-  ultimately have "\<Gamma>' \<turnstile> App (Lam [x].\<gamma><s12>) (\<gamma><s2>) is \<theta><t12[x::=t2]> : T2" 
+  have ih1:"\<And>\<Gamma>' \<gamma> \<theta>. \<Gamma>' \<turnstile> \<gamma> is \<theta> over \<Gamma> \<Longrightarrow> \<Gamma>' \<turnstile> \<gamma><s\<^isub>2> is \<theta><t\<^isub>2> : T\<^isub>1" by fact
+  have ih2:"\<And>\<Gamma>' \<gamma> \<theta>. \<Gamma>' \<turnstile> \<gamma> is \<theta> over (x,T\<^isub>1)#\<Gamma> \<Longrightarrow> \<Gamma>' \<turnstile> \<gamma><s12> is \<theta><t12> : T\<^isub>2" by fact
+  have "\<Gamma>' \<turnstile> \<gamma><s\<^isub>2> is \<theta><t\<^isub>2> : T\<^isub>1" using ih1 h by auto
+  then have "\<Gamma>' \<turnstile> (x,\<gamma><s\<^isub>2>)#\<gamma> is (x,\<theta><t\<^isub>2>)#\<theta> over (x,T\<^isub>1)#\<Gamma>" using equiv_subst_ext h fs by blast
+  then have "\<Gamma>' \<turnstile> (x,\<gamma><s\<^isub>2>)#\<gamma><s12> is (x,\<theta><t\<^isub>2>)#\<theta><t12> : T\<^isub>2" using ih2 by auto
+  then have "\<Gamma>' \<turnstile> \<gamma><s12>[x::=\<gamma><s\<^isub>2>] is \<theta><t12>[x::=\<theta><t\<^isub>2>] : T\<^isub>2" using fs2 psubst_subst_psubst by auto
+  then have "\<Gamma>' \<turnstile> \<gamma><s12>[x::=\<gamma><s\<^isub>2>] is \<theta><t12[x::=t\<^isub>2]> : T\<^isub>2" using fs2 psubst_subst_propagate by auto
+  moreover have "App (Lam [x].\<gamma><s12>) (\<gamma><s\<^isub>2>) \<leadsto> \<gamma><s12>[x::=\<gamma><s\<^isub>2>]" by auto 
+  ultimately have "\<Gamma>' \<turnstile> App (Lam [x].\<gamma><s12>) (\<gamma><s\<^isub>2>) is \<theta><t12[x::=t\<^isub>2]> : T\<^isub>2" 
     using logical_weak_head_closure' by auto
-  then show "\<Gamma>' \<turnstile> \<gamma><App (Lam [x].s12) s2> is \<theta><t12[x::=t2]> : T2" using fs2 by simp
+  then show "\<Gamma>' \<turnstile> \<gamma><App (Lam [x].s12) s\<^isub>2> is \<theta><t12[x::=t\<^isub>2]> : T\<^isub>2" using fs2 by simp
 next
-  case (Q_Ext x \<Gamma> s t T1 T2 \<Gamma>' \<gamma> \<theta>)
+  case (Q_Ext x \<Gamma> s t T\<^isub>1 T\<^isub>2 \<Gamma>' \<gamma> \<theta>)
   have h2:"\<Gamma>' \<turnstile> \<gamma> is \<theta> over \<Gamma>" by fact
   have fs:"x\<sharp>\<Gamma>" "x\<sharp>s" "x\<sharp>t" by fact
-  have ih:"\<And>\<Gamma>' \<gamma> \<theta>. \<Gamma>' \<turnstile> \<gamma> is \<theta> over (x,T1)#\<Gamma> \<Longrightarrow> \<Gamma>' \<turnstile> \<gamma><App s (Var x)> is \<theta><App t (Var x)> : T2" 
+  have ih:"\<And>\<Gamma>' \<gamma> \<theta>. \<Gamma>' \<turnstile> \<gamma> is \<theta> over (x,T\<^isub>1)#\<Gamma> \<Longrightarrow> \<Gamma>' \<turnstile> \<gamma><App s (Var x)> is \<theta><App t (Var x)> : T\<^isub>2" 
     by fact
    {
     fix \<Gamma>'' s' t'
-    assume hsub:"\<Gamma>'\<lless>\<Gamma>''" and hl:"\<Gamma>''\<turnstile> s' is t' : T1"
+    assume hsub:"\<Gamma>'\<lless>\<Gamma>''" and hl:"\<Gamma>''\<turnstile> s' is t' : T\<^isub>1"
     then have "\<Gamma>'' \<turnstile> \<gamma> is \<theta> over \<Gamma>" using h2 logical_subst_monotonicity by blast
-    then have "\<Gamma>'' \<turnstile> (x,s')#\<gamma> is (x,t')#\<theta> over (x,T1)#\<Gamma>" using equiv_subst_ext hl fs by blast
-    then have "\<Gamma>'' \<turnstile> (x,s')#\<gamma><App s (Var x)>  is (x,t')#\<theta><App t (Var x)> : T2" using ih by blast
-    then have "\<Gamma>'' \<turnstile> App (((x,s')#\<gamma>)<s>) (((x,s')#\<gamma>)<(Var x)>) is App ((x,t')#\<theta><t>) ((x,t')#\<theta><(Var x)>) : T2"
+    then have "\<Gamma>'' \<turnstile> (x,s')#\<gamma> is (x,t')#\<theta> over (x,T\<^isub>1)#\<Gamma>" using equiv_subst_ext hl fs by blast
+    then have "\<Gamma>'' \<turnstile> (x,s')#\<gamma><App s (Var x)>  is (x,t')#\<theta><App t (Var x)> : T\<^isub>2" using ih by blast
+    then have "\<Gamma>'' \<turnstile> App (((x,s')#\<gamma>)<s>) (((x,s')#\<gamma>)<(Var x)>) is App ((x,t')#\<theta><t>) ((x,t')#\<theta><(Var x)>) : T\<^isub>2"
       by auto
-    then have "\<Gamma>'' \<turnstile> App ((x,s')#\<gamma><s>) s'  is App ((x,t')#\<theta><t>) t' : T2" by auto
-    then have "\<Gamma>'' \<turnstile> App (\<gamma><s>) s' is App (\<theta><t>) t' : T2" using fs fresh_psubst_simpl by auto
+    then have "\<Gamma>'' \<turnstile> App ((x,s')#\<gamma><s>) s'  is App ((x,t')#\<theta><t>) t' : T\<^isub>2" by auto
+    then have "\<Gamma>'' \<turnstile> App (\<gamma><s>) s' is App (\<theta><t>) t' : T\<^isub>2" using fs fresh_psubst_simpl by auto
   }
   moreover have "valid \<Gamma>'" using h2 by auto
-  ultimately show "\<Gamma>' \<turnstile> \<gamma><s> is \<theta><t> : T1\<rightarrow>T2" by auto
+  ultimately show "\<Gamma>' \<turnstile> \<gamma><s> is \<theta><t> : T\<^isub>1\<rightarrow>T\<^isub>2" by auto
 qed
 
+
 theorem completeness:
-  assumes "\<Gamma> \<turnstile> s == t : T"
-  shows "\<Gamma> \<turnstile> s <=> t : T"
+  assumes "\<Gamma> \<turnstile> s \<equiv> t : T"
+  shows   "\<Gamma> \<turnstile> s \<Leftrightarrow> t : T"
 using assms
 proof -
   {
@@ -1319,16 +1457,17 @@ proof -
   ultimately have "\<Gamma> \<turnstile> [] is [] over \<Gamma>" by auto 
   then have "\<Gamma> \<turnstile> []<s> is []<t> : T" using fundamental_theorem_2 assms by blast
   then have "\<Gamma> \<turnstile> s is t : T" by simp
-  then show  "\<Gamma> \<turnstile> s <=> t : T" using main_lemma by simp
+  then show  "\<Gamma> \<turnstile> s \<Leftrightarrow> t : T" using main_lemma by simp
 qed
 
-(* Soundness is left as an exercise - like in the book - for the avid formalist 
+text{*
+\section{About soundness}
+*}
 
-theorem soundness:
-  shows "\<lbrakk>\<Gamma> \<turnstile> s <=> t : T; \<Gamma> \<turnstile> t : T; \<Gamma> \<turnstile> s : T\<rbrakk> \<Longrightarrow> \<Gamma> \<turnstile> s == t : T"
-  and   "\<lbrakk>\<Gamma> \<turnstile> s \<leftrightarrow> t : T; \<Gamma> \<turnstile> t : T; \<Gamma> \<turnstile> s : T\<rbrakk> \<Longrightarrow> \<Gamma> \<turnstile> s == t : T"
-
-*)
+text {* We leave soundness as an exercise - like in the book :-) \\ 
+ @{prop[mode=IfThen] "\<lbrakk>\<Gamma> \<turnstile> s \<Leftrightarrow> t : T; \<Gamma> \<turnstile> t : T; \<Gamma> \<turnstile> s : T\<rbrakk> \<Longrightarrow> \<Gamma> \<turnstile> s \<equiv> t : T"} \\
+ @{prop "\<lbrakk>\<Gamma> \<turnstile> s \<leftrightarrow> t : T; \<Gamma> \<turnstile> t : T; \<Gamma> \<turnstile> s : T\<rbrakk> \<Longrightarrow> \<Gamma> \<turnstile> s \<equiv> t : T"} 
+*}
 
 end
 
